Updated examples, removed channel invariants that can be generated.

tests/AddDelay.bpl
@@ -56,31 +56,37 @@ procedure Net#anon$3#entry#3()
   assume C#init == C;
   assume C[Net#b] == 1;
   assume M[Net#b][R[Net#b]] == M[Net#c][R[Net#c] - 1];
-  assert {:msg "  Channel invariant might not hold on action entry"} 0 <= C[Net#d];
-  assert {:msg "  Channel invariant might not hold on action entry"} 0 <= R[Net#d];
-  assert {:msg "  Channel invariant might not hold on action entry"} R[Net#c] == 0;
-  assert {:msg "  Channel invariant might not hold on action entry"} 0 <= C[Net#c];
-  assert {:msg "  Channel invariant might not hold on action entry"} 0 <= R[Net#c];
-  assert {:msg "  Channel invariant might not hold on action entry"} 0 <= C[Net#b];
-  assert {:msg "  Channel invariant might not hold on action entry"} 0 <= R[Net#b];
-  assert {:msg "  Channel invariant might not hold on action entry"} (R[Net#a] + C[Net#a]) == C#init[Net#a];
-  assert {:msg "  Channel invariant might not hold on action entry"} 0 <= C[Net#a];
-  assert {:msg "  Channel invariant might not hold on action entry"} 0 <= R[Net#a];
-  assert {:msg "  17.15: Channel invariant might not hold on action entry"} (R[Net#c] + C[Net#c]) == R[Net#a];
-  assert {:msg "  18.15: Channel invariant might not hold on action entry"} (R[Net#c] + C[Net#c]) == R[Net#b];
-  assert {:msg "  19.15: Channel invariant might not hold on action entry"} (R[Net#d] + C[Net#d]) == R[Net#a];
-  assert {:msg "  20.15: Channel invariant might not hold on action entry"} (R[Net#d] + C[Net#d]) == R[Net#b];
-  assert {:msg "  21.15: Channel invariant might not hold on action entry"} (R[Net#b] + C[Net#b]) == (R[Net#d] + 1);
-  assert {:msg "  22.16: Channel invariant might not hold on action entry"} (forall i: int :: 
-    (0 <= i) && (i < (R[Net#c] + C[Net#c])) ==> (M[Net#c][i] == (M[Net#a][i] + M[Net#b][i]))
+  assert {:msg "  Channel invariant might not hold on action entry (generated #0 )"} (forall idx$: int :: 
+    (0 <= idx$) && (idx$ < ((R[Net#b] + C[Net#b]) - 1)) ==> (M[Net#b][(idx$ + 1) - 0] == M[Net#d][idx$ - 0])
   );
-  assert {:msg "  23.16: Channel invariant might not hold on action entry"} (forall i: int :: 
-    (0 <= i) && (i < (R[Net#d] + C[Net#d])) ==> (M[Net#d][i] == (M[Net#a][i] + M[Net#b][i]))
+  assert {:msg "  Channel invariant might not hold on action entry (generated #1 )"} R[Net#d] == ((R[Net#b] + C[Net#b]) - 1);
+  assert {:msg "  Channel invariant might not hold on action entry (generated #2 )"} (forall idx$: int :: 
+    (0 <= idx$) && (idx$ < (R[Net#d] + C[Net#d])) ==> (M[Net#d][idx$ - 0] == (M[Net#a][idx$ - 0] + M[Net#b][idx$ - 0]))
   );
-  assert {:msg "  24.16: Channel invariant might not hold on action entry"} (forall i: int :: 
-    (1 <= i) && (i < (R[Net#b] + C[Net#b])) ==> (M[Net#b][i] == M[Net#d][i - 1])
+  assert {:msg "  Channel invariant might not hold on action entry (generated #3 )"} R[Net#b] == (R[Net#d] + C[Net#d]);
+  assert {:msg "  Channel invariant might not hold on action entry (generated #4 )"} (forall idx$: int :: 
+    (0 <= idx$) && (idx$ < (R[Net#c] + C[Net#c])) ==> (M[Net#c][idx$ - 0] == (M[Net#a][idx$ - 0] + M[Net#b][idx$ - 0]))
   );
-  assert {:msg "  25.15: Channel invariant might not hold on action entry"} M[Net#b][0] == M[Net#c][-1];
+  assert {:msg "  Channel invariant might not hold on action entry (generated #5 )"} R[Net#b] == (R[Net#c] + C[Net#c]);
+  assert {:msg "  Channel invariant might not hold on action entry (generated #6 )"} (forall idx$: int :: 
+    (0 <= idx$) && (idx$ < (R[Net#d] + C[Net#d])) ==> (M[Net#d][idx$ - 0] == (M[Net#a][idx$ - 0] + M[Net#b][idx$ - 0]))
+  );
+  assert {:msg "  Channel invariant might not hold on action entry (generated #7 )"} R[Net#a] == (R[Net#d] + C[Net#d]);
+  assert {:msg "  Channel invariant might not hold on action entry (generated #8 )"} (forall idx$: int :: 
+    (0 <= idx$) && (idx$ < (R[Net#c] + C[Net#c])) ==> (M[Net#c][idx$ - 0] == (M[Net#a][idx$ - 0] + M[Net#b][idx$ - 0]))
+  );
+  assert {:msg "  Channel invariant might not hold on action entry (generated #9 )"} R[Net#a] == (R[Net#c] + C[Net#c]);
+  assert {:msg "  Channel invariant might not hold on action entry (generated #10 )"} 0 <= C[Net#d];
+  assert {:msg "  Channel invariant might not hold on action entry (generated #11 )"} 0 <= R[Net#d];
+  assert {:msg "  Channel invariant might not hold on action entry (generated #12 )"} R[Net#c] == 0;
+  assert {:msg "  Channel invariant might not hold on action entry (generated #13 )"} 0 <= C[Net#c];
+  assert {:msg "  Channel invariant might not hold on action entry (generated #14 )"} 0 <= R[Net#c];
+  assert {:msg "  Channel invariant might not hold on action entry (generated #15 )"} 0 <= C[Net#b];
+  assert {:msg "  Channel invariant might not hold on action entry (generated #16 )"} 0 <= R[Net#b];
+  assert {:msg "  Channel invariant might not hold on action entry (generated #17 )"} (R[Net#a] + C[Net#a]) == C#init[Net#a];
+  assert {:msg "  Channel invariant might not hold on action entry (generated #18 )"} 0 <= C[Net#a];
+  assert {:msg "  Channel invariant might not hold on action entry (generated #19 )"} 0 <= R[Net#a];
+  assert {:msg "  18.3: Channel invariant might not hold on action entry"} M[Net#b][0] == M[Net#c][-1];
 }
 procedure Net#anon$3#Add#anon$0#4()
   modifies C, R, M, St;
@@ -91,6 +97,26 @@ procedure Net#anon$3#Add#anon$0#4()
   assume C#init[Net#a] == 1;
   assume C#init[Net#c] == 0;
   assume C#init[Net#d] == 0;
+  assume (forall idx$: int :: 
+    (0 <= idx$) && (idx$ < ((R[Net#b] + C[Net#b]) - 1)) ==> (M[Net#b][(idx$ + 1) - 0] == M[Net#d][idx$ - 0])
+  );
+  assume R[Net#d] == ((R[Net#b] + C[Net#b]) - 1);
+  assume (forall idx$: int :: 
+    (0 <= idx$) && (idx$ < (R[Net#d] + C[Net#d])) ==> (M[Net#d][idx$ - 0] == (M[Net#a][idx$ - 0] + M[Net#b][idx$ - 0]))
+  );
+  assume R[Net#b] == (R[Net#d] + C[Net#d]);
+  assume (forall idx$: int :: 
+    (0 <= idx$) && (idx$ < (R[Net#c] + C[Net#c])) ==> (M[Net#c][idx$ - 0] == (M[Net#a][idx$ - 0] + M[Net#b][idx$ - 0]))
+  );
+  assume R[Net#b] == (R[Net#c] + C[Net#c]);
+  assume (forall idx$: int :: 
+    (0 <= idx$) && (idx$ < (R[Net#d] + C[Net#d])) ==> (M[Net#d][idx$ - 0] == (M[Net#a][idx$ - 0] + M[Net#b][idx$ - 0]))
+  );
+  assume R[Net#a] == (R[Net#d] + C[Net#d]);
+  assume (forall idx$: int :: 
+    (0 <= idx$) && (idx$ < (R[Net#c] + C[Net#c])) ==> (M[Net#c][idx$ - 0] == (M[Net#a][idx$ - 0] + M[Net#b][idx$ - 0]))
+  );
+  assume R[Net#a] == (R[Net#c] + C[Net#c]);
   assume 0 <= C[Net#d];
   assume 0 <= R[Net#d];
   assume R[Net#c] == 0;
@@ -101,20 +127,6 @@ procedure Net#anon$3#Add#anon$0#4()
   assume (R[Net#a] + C[Net#a]) == C#init[Net#a];
   assume 0 <= C[Net#a];
   assume 0 <= R[Net#a];
-  assume (R[Net#c] + C[Net#c]) == R[Net#a];
-  assume (R[Net#c] + C[Net#c]) == R[Net#b];
-  assume (R[Net#d] + C[Net#d]) == R[Net#a];
-  assume (R[Net#d] + C[Net#d]) == R[Net#b];
-  assume (R[Net#b] + C[Net#b]) == (R[Net#d] + 1);
-  assume (forall i: int :: 
-    (0 <= i) && (i < (R[Net#c] + C[Net#c])) ==> (M[Net#c][i] == (M[Net#a][i] + M[Net#b][i]))
-  );
-  assume (forall i: int :: 
-    (0 <= i) && (i < (R[Net#d] + C[Net#d])) ==> (M[Net#d][i] == (M[Net#a][i] + M[Net#b][i]))
-  );
-  assume (forall i: int :: 
-    (1 <= i) && (i < (R[Net#b] + C[Net#b])) ==> (M[Net#b][i] == M[Net#d][i - 1])
-  );
   assume M[Net#b][0] == M[Net#c][-1];
   assume true;
   assume (1 <= C[Net#a]) && (1 <= C[Net#b]);
@@ -128,31 +140,37 @@ procedure Net#anon$3#Add#anon$0#4()
   C[Net#c] := C[Net#c] + 1;
   M[Net#d][R[Net#d] + C[Net#d]] := in1#i + in2#j;
   C[Net#d] := C[Net#d] + 1;
-  assert {:msg "  Sub-actor action at 3.3 might not preserve the channel invariant"} 0 <= C[Net#d];
-  assert {:msg "  Sub-actor action at 3.3 might not preserve the channel invariant"} 0 <= R[Net#d];
-  assert {:msg "  Sub-actor action at 3.3 might not preserve the channel invariant"} R[Net#c] == 0;
-  assert {:msg "  Sub-actor action at 3.3 might not preserve the channel invariant"} 0 <= C[Net#c];
-  assert {:msg "  Sub-actor action at 3.3 might not preserve the channel invariant"} 0 <= R[Net#c];
-  assert {:msg "  Sub-actor action at 3.3 might not preserve the channel invariant"} 0 <= C[Net#b];
-  assert {:msg "  Sub-actor action at 3.3 might not preserve the channel invariant"} 0 <= R[Net#b];
-  assert {:msg "  Sub-actor action at 3.3 might not preserve the channel invariant"} (R[Net#a] + C[Net#a]) == C#init[Net#a];
-  assert {:msg "  Sub-actor action at 3.3 might not preserve the channel invariant"} 0 <= C[Net#a];
-  assert {:msg "  Sub-actor action at 3.3 might not preserve the channel invariant"} 0 <= R[Net#a];
-  assert {:msg "  17.15: Sub-actor action at 3.3 might not preserve the channel invariant"} (R[Net#c] + C[Net#c]) == R[Net#a];
-  assert {:msg "  18.15: Sub-actor action at 3.3 might not preserve the channel invariant"} (R[Net#c] + C[Net#c]) == R[Net#b];
-  assert {:msg "  19.15: Sub-actor action at 3.3 might not preserve the channel invariant"} (R[Net#d] + C[Net#d]) == R[Net#a];
-  assert {:msg "  20.15: Sub-actor action at 3.3 might not preserve the channel invariant"} (R[Net#d] + C[Net#d]) == R[Net#b];
-  assert {:msg "  21.15: Sub-actor action at 3.3 might not preserve the channel invariant"} (R[Net#b] + C[Net#b]) == (R[Net#d] + 1);
-  assert {:msg "  22.16: Sub-actor action at 3.3 might not preserve the channel invariant"} (forall i: int :: 
-    (0 <= i) && (i < (R[Net#c] + C[Net#c])) ==> (M[Net#c][i] == (M[Net#a][i] + M[Net#b][i]))
+  assert {:msg "  Sub-actor action at 3.3 might not preserve the channel invariant (generated #20)"} (forall idx$: int :: 
+    (0 <= idx$) && (idx$ < ((R[Net#b] + C[Net#b]) - 1)) ==> (M[Net#b][(idx$ + 1) - 0] == M[Net#d][idx$ - 0])
   );
-  assert {:msg "  23.16: Sub-actor action at 3.3 might not preserve the channel invariant"} (forall i: int :: 
-    (0 <= i) && (i < (R[Net#d] + C[Net#d])) ==> (M[Net#d][i] == (M[Net#a][i] + M[Net#b][i]))
+  assert {:msg "  Sub-actor action at 3.3 might not preserve the channel invariant (generated #21)"} R[Net#d] == ((R[Net#b] + C[Net#b]) - 1);
+  assert {:msg "  Sub-actor action at 3.3 might not preserve the channel invariant (generated #22)"} (forall idx$: int :: 
+    (0 <= idx$) && (idx$ < (R[Net#d] + C[Net#d])) ==> (M[Net#d][idx$ - 0] == (M[Net#a][idx$ - 0] + M[Net#b][idx$ - 0]))
   );
-  assert {:msg "  24.16: Sub-actor action at 3.3 might not preserve the channel invariant"} (forall i: int :: 
-    (1 <= i) && (i < (R[Net#b] + C[Net#b])) ==> (M[Net#b][i] == M[Net#d][i - 1])
+  assert {:msg "  Sub-actor action at 3.3 might not preserve the channel invariant (generated #23)"} R[Net#b] == (R[Net#d] + C[Net#d]);
+  assert {:msg "  Sub-actor action at 3.3 might not preserve the channel invariant (generated #24)"} (forall idx$: int :: 
+    (0 <= idx$) && (idx$ < (R[Net#c] + C[Net#c])) ==> (M[Net#c][idx$ - 0] == (M[Net#a][idx$ - 0] + M[Net#b][idx$ - 0]))
   );
-  assert {:msg "  25.15: Sub-actor action at 3.3 might not preserve the channel invariant"} M[Net#b][0] == M[Net#c][-1];
+  assert {:msg "  Sub-actor action at 3.3 might not preserve the channel invariant (generated #25)"} R[Net#b] == (R[Net#c] + C[Net#c]);
+  assert {:msg "  Sub-actor action at 3.3 might not preserve the channel invariant (generated #26)"} (forall idx$: int :: 
+    (0 <= idx$) && (idx$ < (R[Net#d] + C[Net#d])) ==> (M[Net#d][idx$ - 0] == (M[Net#a][idx$ - 0] + M[Net#b][idx$ - 0]))
+  );
+  assert {:msg "  Sub-actor action at 3.3 might not preserve the channel invariant (generated #27)"} R[Net#a] == (R[Net#d] + C[Net#d]);
+  assert {:msg "  Sub-actor action at 3.3 might not preserve the channel invariant (generated #28)"} (forall idx$: int :: 
+    (0 <= idx$) && (idx$ < (R[Net#c] + C[Net#c])) ==> (M[Net#c][idx$ - 0] == (M[Net#a][idx$ - 0] + M[Net#b][idx$ - 0]))
+  );
+  assert {:msg "  Sub-actor action at 3.3 might not preserve the channel invariant (generated #29)"} R[Net#a] == (R[Net#c] + C[Net#c]);
+  assert {:msg "  Sub-actor action at 3.3 might not preserve the channel invariant (generated #30)"} 0 <= C[Net#d];
+  assert {:msg "  Sub-actor action at 3.3 might not preserve the channel invariant (generated #31)"} 0 <= R[Net#d];
+  assert {:msg "  Sub-actor action at 3.3 might not preserve the channel invariant (generated #32)"} R[Net#c] == 0;
+  assert {:msg "  Sub-actor action at 3.3 might not preserve the channel invariant (generated #33)"} 0 <= C[Net#c];
+  assert {:msg "  Sub-actor action at 3.3 might not preserve the channel invariant (generated #34)"} 0 <= R[Net#c];
+  assert {:msg "  Sub-actor action at 3.3 might not preserve the channel invariant (generated #35)"} 0 <= C[Net#b];
+  assert {:msg "  Sub-actor action at 3.3 might not preserve the channel invariant (generated #36)"} 0 <= R[Net#b];
+  assert {:msg "  Sub-actor action at 3.3 might not preserve the channel invariant (generated #37)"} (R[Net#a] + C[Net#a]) == C#init[Net#a];
+  assert {:msg "  Sub-actor action at 3.3 might not preserve the channel invariant (generated #38)"} 0 <= C[Net#a];
+  assert {:msg "  Sub-actor action at 3.3 might not preserve the channel invariant (generated #39)"} 0 <= R[Net#a];
+  assert {:msg "  18.3: Sub-actor action at 3.3 might not preserve the channel invariant"} M[Net#b][0] == M[Net#c][-1];
 }
 procedure Net#anon$3#Delay#anon$2#5()
   modifies C, R, M, St;
@@ -164,6 +182,26 @@ procedure Net#anon$3#Delay#anon$2#5()
   assume C#init[Net#a] == 1;
   assume C#init[Net#c] == 0;
   assume C#init[Net#d] == 0;
+  assume (forall idx$: int :: 
+    (0 <= idx$) && (idx$ < ((R[Net#b] + C[Net#b]) - 1)) ==> (M[Net#b][(idx$ + 1) - 0] == M[Net#d][idx$ - 0])
+  );
+  assume R[Net#d] == ((R[Net#b] + C[Net#b]) - 1);
+  assume (forall idx$: int :: 
+    (0 <= idx$) && (idx$ < (R[Net#d] + C[Net#d])) ==> (M[Net#d][idx$ - 0] == (M[Net#a][idx$ - 0] + M[Net#b][idx$ - 0]))
+  );
+  assume R[Net#b] == (R[Net#d] + C[Net#d]);
+  assume (forall idx$: int :: 
+    (0 <= idx$) && (idx$ < (R[Net#c] + C[Net#c])) ==> (M[Net#c][idx$ - 0] == (M[Net#a][idx$ - 0] + M[Net#b][idx$ - 0]))
+  );
+  assume R[Net#b] == (R[Net#c] + C[Net#c]);
+  assume (forall idx$: int :: 
+    (0 <= idx$) && (idx$ < (R[Net#d] + C[Net#d])) ==> (M[Net#d][idx$ - 0] == (M[Net#a][idx$ - 0] + M[Net#b][idx$ - 0]))
+  );
+  assume R[Net#a] == (R[Net#d] + C[Net#d]);
+  assume (forall idx$: int :: 
+    (0 <= idx$) && (idx$ < (R[Net#c] + C[Net#c])) ==> (M[Net#c][idx$ - 0] == (M[Net#a][idx$ - 0] + M[Net#b][idx$ - 0]))
+  );
+  assume R[Net#a] == (R[Net#c] + C[Net#c]);
   assume 0 <= C[Net#d];
   assume 0 <= R[Net#d];
   assume R[Net#c] == 0;
@@ -174,20 +212,6 @@ procedure Net#anon$3#Delay#anon$2#5()
   assume (R[Net#a] + C[Net#a]) == C#init[Net#a];
   assume 0 <= C[Net#a];
   assume 0 <= R[Net#a];
-  assume (R[Net#c] + C[Net#c]) == R[Net#a];
-  assume (R[Net#c] + C[Net#c]) == R[Net#b];
-  assume (R[Net#d] + C[Net#d]) == R[Net#a];
-  assume (R[Net#d] + C[Net#d]) == R[Net#b];
-  assume (R[Net#b] + C[Net#b]) == (R[Net#d] + 1);
-  assume (forall i: int :: 
-    (0 <= i) && (i < (R[Net#c] + C[Net#c])) ==> (M[Net#c][i] == (M[Net#a][i] + M[Net#b][i]))
-  );
-  assume (forall i: int :: 
-    (0 <= i) && (i < (R[Net#d] + C[Net#d])) ==> (M[Net#d][i] == (M[Net#a][i] + M[Net#b][i]))
-  );
-  assume (forall i: int :: 
-    (1 <= i) && (i < (R[Net#b] + C[Net#b])) ==> (M[Net#b][i] == M[Net#d][i - 1])
-  );
   assume M[Net#b][0] == M[Net#c][-1];
   assume true;
   assume 1 <= C[Net#d];
@@ -196,31 +220,37 @@ procedure Net#anon$3#Delay#anon$2#5()
   C[Net#d] := C[Net#d] - 1;
   M[Net#b][R[Net#b] + C[Net#b]] := in#i;
   C[Net#b] := C[Net#b] + 1;
-  assert {:msg "  Sub-actor action at 8.3 might not preserve the channel invariant"} 0 <= C[Net#d];
-  assert {:msg "  Sub-actor action at 8.3 might not preserve the channel invariant"} 0 <= R[Net#d];
-  assert {:msg "  Sub-actor action at 8.3 might not preserve the channel invariant"} R[Net#c] == 0;
-  assert {:msg "  Sub-actor action at 8.3 might not preserve the channel invariant"} 0 <= C[Net#c];
-  assert {:msg "  Sub-actor action at 8.3 might not preserve the channel invariant"} 0 <= R[Net#c];
-  assert {:msg "  Sub-actor action at 8.3 might not preserve the channel invariant"} 0 <= C[Net#b];
-  assert {:msg "  Sub-actor action at 8.3 might not preserve the channel invariant"} 0 <= R[Net#b];
-  assert {:msg "  Sub-actor action at 8.3 might not preserve the channel invariant"} (R[Net#a] + C[Net#a]) == C#init[Net#a];
-  assert {:msg "  Sub-actor action at 8.3 might not preserve the channel invariant"} 0 <= C[Net#a];
-  assert {:msg "  Sub-actor action at 8.3 might not preserve the channel invariant"} 0 <= R[Net#a];
-  assert {:msg "  17.15: Sub-actor action at 8.3 might not preserve the channel invariant"} (R[Net#c] + C[Net#c]) == R[Net#a];
-  assert {:msg "  18.15: Sub-actor action at 8.3 might not preserve the channel invariant"} (R[Net#c] + C[Net#c]) == R[Net#b];
-  assert {:msg "  19.15: Sub-actor action at 8.3 might not preserve the channel invariant"} (R[Net#d] + C[Net#d]) == R[Net#a];
-  assert {:msg "  20.15: Sub-actor action at 8.3 might not preserve the channel invariant"} (R[Net#d] + C[Net#d]) == R[Net#b];
-  assert {:msg "  21.15: Sub-actor action at 8.3 might not preserve the channel invariant"} (R[Net#b] + C[Net#b]) == (R[Net#d] + 1);
-  assert {:msg "  22.16: Sub-actor action at 8.3 might not preserve the channel invariant"} (forall i: int :: 
-    (0 <= i) && (i < (R[Net#c] + C[Net#c])) ==> (M[Net#c][i] == (M[Net#a][i] + M[Net#b][i]))
+  assert {:msg "  Sub-actor action at 9.3 might not preserve the channel invariant (generated #40)"} (forall idx$: int :: 
+    (0 <= idx$) && (idx$ < ((R[Net#b] + C[Net#b]) - 1)) ==> (M[Net#b][(idx$ + 1) - 0] == M[Net#d][idx$ - 0])
   );
-  assert {:msg "  23.16: Sub-actor action at 8.3 might not preserve the channel invariant"} (forall i: int :: 
-    (0 <= i) && (i < (R[Net#d] + C[Net#d])) ==> (M[Net#d][i] == (M[Net#a][i] + M[Net#b][i]))
+  assert {:msg "  Sub-actor action at 9.3 might not preserve the channel invariant (generated #41)"} R[Net#d] == ((R[Net#b] + C[Net#b]) - 1);
+  assert {:msg "  Sub-actor action at 9.3 might not preserve the channel invariant (generated #42)"} (forall idx$: int :: 
+    (0 <= idx$) && (idx$ < (R[Net#d] + C[Net#d])) ==> (M[Net#d][idx$ - 0] == (M[Net#a][idx$ - 0] + M[Net#b][idx$ - 0]))
   );
-  assert {:msg "  24.16: Sub-actor action at 8.3 might not preserve the channel invariant"} (forall i: int :: 
-    (1 <= i) && (i < (R[Net#b] + C[Net#b])) ==> (M[Net#b][i] == M[Net#d][i - 1])
+  assert {:msg "  Sub-actor action at 9.3 might not preserve the channel invariant (generated #43)"} R[Net#b] == (R[Net#d] + C[Net#d]);
+  assert {:msg "  Sub-actor action at 9.3 might not preserve the channel invariant (generated #44)"} (forall idx$: int :: 
+    (0 <= idx$) && (idx$ < (R[Net#c] + C[Net#c])) ==> (M[Net#c][idx$ - 0] == (M[Net#a][idx$ - 0] + M[Net#b][idx$ - 0]))
   );
-  assert {:msg "  25.15: Sub-actor action at 8.3 might not preserve the channel invariant"} M[Net#b][0] == M[Net#c][-1];
+  assert {:msg "  Sub-actor action at 9.3 might not preserve the channel invariant (generated #45)"} R[Net#b] == (R[Net#c] + C[Net#c]);
+  assert {:msg "  Sub-actor action at 9.3 might not preserve the channel invariant (generated #46)"} (forall idx$: int :: 
+    (0 <= idx$) && (idx$ < (R[Net#d] + C[Net#d])) ==> (M[Net#d][idx$ - 0] == (M[Net#a][idx$ - 0] + M[Net#b][idx$ - 0]))
+  );
+  assert {:msg "  Sub-actor action at 9.3 might not preserve the channel invariant (generated #47)"} R[Net#a] == (R[Net#d] + C[Net#d]);
+  assert {:msg "  Sub-actor action at 9.3 might not preserve the channel invariant (generated #48)"} (forall idx$: int :: 
+    (0 <= idx$) && (idx$ < (R[Net#c] + C[Net#c])) ==> (M[Net#c][idx$ - 0] == (M[Net#a][idx$ - 0] + M[Net#b][idx$ - 0]))
+  );
+  assert {:msg "  Sub-actor action at 9.3 might not preserve the channel invariant (generated #49)"} R[Net#a] == (R[Net#c] + C[Net#c]);
+  assert {:msg "  Sub-actor action at 9.3 might not preserve the channel invariant (generated #50)"} 0 <= C[Net#d];
+  assert {:msg "  Sub-actor action at 9.3 might not preserve the channel invariant (generated #51)"} 0 <= R[Net#d];
+  assert {:msg "  Sub-actor action at 9.3 might not preserve the channel invariant (generated #52)"} R[Net#c] == 0;
+  assert {:msg "  Sub-actor action at 9.3 might not preserve the channel invariant (generated #53)"} 0 <= C[Net#c];
+  assert {:msg "  Sub-actor action at 9.3 might not preserve the channel invariant (generated #54)"} 0 <= R[Net#c];
+  assert {:msg "  Sub-actor action at 9.3 might not preserve the channel invariant (generated #55)"} 0 <= C[Net#b];
+  assert {:msg "  Sub-actor action at 9.3 might not preserve the channel invariant (generated #56)"} 0 <= R[Net#b];
+  assert {:msg "  Sub-actor action at 9.3 might not preserve the channel invariant (generated #57)"} (R[Net#a] + C[Net#a]) == C#init[Net#a];
+  assert {:msg "  Sub-actor action at 9.3 might not preserve the channel invariant (generated #58)"} 0 <= C[Net#a];
+  assert {:msg "  Sub-actor action at 9.3 might not preserve the channel invariant (generated #59)"} 0 <= R[Net#a];
+  assert {:msg "  18.3: Sub-actor action at 9.3 might not preserve the channel invariant"} M[Net#b][0] == M[Net#c][-1];
 }
 procedure Net#anon$3#exit#6()
   modifies C, R, M, St;
@@ -228,6 +258,26 @@ procedure Net#anon$3#exit#6()
   assume C#init[Net#a] == 1;
   assume C#init[Net#c] == 0;
   assume C#init[Net#d] == 0;
+  assume (forall idx$: int :: 
+    (0 <= idx$) && (idx$ < ((R[Net#b] + C[Net#b]) - 1)) ==> (M[Net#b][(idx$ + 1) - 0] == M[Net#d][idx$ - 0])
+  );
+  assume R[Net#d] == ((R[Net#b] + C[Net#b]) - 1);
+  assume (forall idx$: int :: 
+    (0 <= idx$) && (idx$ < (R[Net#d] + C[Net#d])) ==> (M[Net#d][idx$ - 0] == (M[Net#a][idx$ - 0] + M[Net#b][idx$ - 0]))
+  );
+  assume R[Net#b] == (R[Net#d] + C[Net#d]);
+  assume (forall idx$: int :: 
+    (0 <= idx$) && (idx$ < (R[Net#c] + C[Net#c])) ==> (M[Net#c][idx$ - 0] == (M[Net#a][idx$ - 0] + M[Net#b][idx$ - 0]))
+  );
+  assume R[Net#b] == (R[Net#c] + C[Net#c]);
+  assume (forall idx$: int :: 
+    (0 <= idx$) && (idx$ < (R[Net#d] + C[Net#d])) ==> (M[Net#d][idx$ - 0] == (M[Net#a][idx$ - 0] + M[Net#b][idx$ - 0]))
+  );
+  assume R[Net#a] == (R[Net#d] + C[Net#d]);
+  assume (forall idx$: int :: 
+    (0 <= idx$) && (idx$ < (R[Net#c] + C[Net#c])) ==> (M[Net#c][idx$ - 0] == (M[Net#a][idx$ - 0] + M[Net#b][idx$ - 0]))
+  );
+  assume R[Net#a] == (R[Net#c] + C[Net#c]);
   assume 0 <= C[Net#d];
   assume 0 <= R[Net#d];
   assume R[Net#c] == 0;
@@ -238,28 +288,14 @@ procedure Net#anon$3#exit#6()
   assume (R[Net#a] + C[Net#a]) == C#init[Net#a];
   assume 0 <= C[Net#a];
   assume 0 <= R[Net#a];
-  assume (R[Net#c] + C[Net#c]) == R[Net#a];
-  assume (R[Net#c] + C[Net#c]) == R[Net#b];
-  assume (R[Net#d] + C[Net#d]) == R[Net#a];
-  assume (R[Net#d] + C[Net#d]) == R[Net#b];
-  assume (R[Net#b] + C[Net#b]) == (R[Net#d] + 1);
-  assume (forall i: int :: 
-    (0 <= i) && (i < (R[Net#c] + C[Net#c])) ==> (M[Net#c][i] == (M[Net#a][i] + M[Net#b][i]))
-  );
-  assume (forall i: int :: 
-    (0 <= i) && (i < (R[Net#d] + C[Net#d])) ==> (M[Net#d][i] == (M[Net#a][i] + M[Net#b][i]))
-  );
-  assume (forall i: int :: 
-    (1 <= i) && (i < (R[Net#b] + C[Net#b])) ==> (M[Net#b][i] == M[Net#d][i - 1])
-  );
   assume M[Net#b][0] == M[Net#c][-1];
   assume !(((1 <= C[Net#a]) && (1 <= C[Net#b])) || (1 <= C[Net#d]));
-  assert {:msg "  12.3: The network might leave unread tokens on channel a"} C[Net#a] == 0;
-  assert {:msg "  12.3: The network might not produce the specified number of tokens on output out"} C[Net#c] == 1;
-  assert {:msg "  12.3: The network might leave unread tokens on channel d"} C[Net#d] == 0;
-  assert {:msg "  12.26: Network output might not conform to specified action output"} M[Net#c][0] == (M[Net#c][R[Net#c] - 1] + M[Net#a][0]);
+  assert {:msg "  13.3: The network might leave unread tokens on channel a"} C[Net#a] == 0;
+  assert {:msg "  13.3: The network might not produce the specified number of tokens on output out"} C[Net#c] == 1;
+  assert {:msg "  13.3: The network might leave unread tokens on channel d"} C[Net#d] == 0;
+  assert {:msg "  13.26: Network output might not conform to specified action output"} M[Net#c][0] == (M[Net#c][R[Net#c] - 1] + M[Net#a][0]);
   R[Net#c] := R[Net#c] + C[Net#c];
   C[Net#c] := 0;
-  assert {:msg "  14.13: The network might not preserve the network invariant"} C[Net#b] == 1;
-  assert {:msg "  15.13: The network might not preserve the network invariant"} M[Net#b][R[Net#b]] == M[Net#c][R[Net#c] - 1];
+  assert {:msg "  15.3: The network might not preserve the network invariant"} C[Net#b] == 1;
+  assert {:msg "  16.3: The network might not preserve the network invariant"} M[Net#b][R[Net#b]] == M[Net#c][R[Net#c] - 1];
 }
