tests/DataDependent.bpl
@@ -64,28 +64,28 @@ procedure Net#anon$3#entry#3()
   assume R[Net#d] == 0;
   assume (M[Net#a][0] < 0) && (M[Net#a][1] > 0);
   assume C#init == C;
-  assert {:msg "  Channel invariant might not hold on action entry (generated)"} R[Net#a] == (R[Net#b] + C[Net#b]);
-  assert {:msg "  Channel invariant might not hold on action entry (generated)"} R[Net#d] == 0;
-  assert {:msg "  Channel invariant might not hold on action entry (generated)"} 0 <= C[Net#d];
-  assert {:msg "  Channel invariant might not hold on action entry (generated)"} 0 <= R[Net#d];
-  assert {:msg "  Channel invariant might not hold on action entry (generated)"} R[Net#c] == 0;
-  assert {:msg "  Channel invariant might not hold on action entry (generated)"} 0 <= C[Net#c];
-  assert {:msg "  Channel invariant might not hold on action entry (generated)"} 0 <= R[Net#c];
-  assert {:msg "  Channel invariant might not hold on action entry (generated)"} 0 <= C[Net#b];
-  assert {:msg "  Channel invariant might not hold on action entry (generated)"} 0 <= R[Net#b];
-  assert {:msg "  Channel invariant might not hold on action entry (generated)"} (R[Net#a] + C[Net#a]) == C#init[Net#a];
-  assert {:msg "  Channel invariant might not hold on action entry (generated)"} 0 <= C[Net#a];
-  assert {:msg "  Channel invariant might not hold on action entry (generated)"} 0 <= R[Net#a];
+  assert {:msg "  Channel invariant might not hold on action entry (generated #0 )"} 0 <= R[Net#a];
+  assert {:msg "  Channel invariant might not hold on action entry (generated #1 )"} 0 <= C[Net#a];
+  assert {:msg "  Channel invariant might not hold on action entry (generated #2 )"} (R[Net#a] + C[Net#a]) == C#init[Net#a];
+  assert {:msg "  Channel invariant might not hold on action entry (generated #3 )"} 0 <= R[Net#b];
+  assert {:msg "  Channel invariant might not hold on action entry (generated #4 )"} 0 <= C[Net#b];
+  assert {:msg "  Channel invariant might not hold on action entry (generated #5 )"} 0 <= R[Net#c];
+  assert {:msg "  Channel invariant might not hold on action entry (generated #6 )"} 0 <= C[Net#c];
+  assert {:msg "  Channel invariant might not hold on action entry (generated #7 )"} R[Net#c] == 0;
+  assert {:msg "  Channel invariant might not hold on action entry (generated #8 )"} 0 <= R[Net#d];
+  assert {:msg "  Channel invariant might not hold on action entry (generated #9 )"} 0 <= C[Net#d];
+  assert {:msg "  Channel invariant might not hold on action entry (generated #10 )"} R[Net#d] == 0;
+  assert {:msg "  Channel invariant might not hold on action entry (generated #11 )"} R[Net#a] == (R[Net#b] + C[Net#b]);
+  assert {:msg "  Channel invariant might not hold on action entry (generated #12 )"} (forall idx: int :: 
+    (0 <= idx) && (idx < (R[Net#b] + C[Net#b])) ==> (M[Net#b][idx] == M[Net#a][idx])
+  );
   assert {:msg "  20.3: Channel invariant might not hold on action entry"} (M[Net#a][0] < 0) && (M[Net#a][1] > 0);
   assert {:msg "  21.3: Channel invariant might not hold on action entry"} (R[Net#d] + C[Net#d]) == AT#Div(R[Net#b] + 1, 2);
   assert {:msg "  22.3: Channel invariant might not hold on action entry"} (R[Net#c] + C[Net#c]) == AT#Div(R[Net#b], 2);
   assert {:msg "  23.3: Channel invariant might not hold on action entry"} (forall i: int :: 
-    (0 <= i) && (i < (R[Net#b] + C[Net#b])) ==> (M[Net#b][i] == M[Net#a][i])
-  );
-  assert {:msg "  24.3: Channel invariant might not hold on action entry"} (forall i: int :: 
     (0 <= i) && (i < R[Net#b]) && (AT#Mod(i, 2) == 0) ==> (M[Net#b][i] == M[Net#d][AT#Div(i, 2)])
   );
-  assert {:msg "  25.3: Channel invariant might not hold on action entry"} (forall i: int :: 
+  assert {:msg "  24.3: Channel invariant might not hold on action entry"} (forall i: int :: 
     (0 <= i) && (i < R[Net#b]) && (AT#Mod(i, 2) == 1) ==> (M[Net#b][i] == M[Net#c][AT#Div(i, 2)])
   );
 }
@@ -98,24 +98,24 @@ procedure Net#anon$3#Repeater#anon$0#4()
   assume C#init[Net#b] == 0;
   assume C#init[Net#c] == 0;
   assume C#init[Net#d] == 0;
-  assume R[Net#a] == (R[Net#b] + C[Net#b]);
-  assume R[Net#d] == 0;
-  assume 0 <= C[Net#d];
-  assume 0 <= R[Net#d];
-  assume R[Net#c] == 0;
-  assume 0 <= C[Net#c];
-  assume 0 <= R[Net#c];
-  assume 0 <= C[Net#b];
-  assume 0 <= R[Net#b];
-  assume (R[Net#a] + C[Net#a]) == C#init[Net#a];
-  assume 0 <= C[Net#a];
   assume 0 <= R[Net#a];
+  assume 0 <= C[Net#a];
+  assume (R[Net#a] + C[Net#a]) == C#init[Net#a];
+  assume 0 <= R[Net#b];
+  assume 0 <= C[Net#b];
+  assume 0 <= R[Net#c];
+  assume 0 <= C[Net#c];
+  assume R[Net#c] == 0;
+  assume 0 <= R[Net#d];
+  assume 0 <= C[Net#d];
+  assume R[Net#d] == 0;
+  assume R[Net#a] == (R[Net#b] + C[Net#b]);
+  assume (forall idx: int :: 
+    (0 <= idx) && (idx < (R[Net#b] + C[Net#b])) ==> (M[Net#b][idx] == M[Net#a][idx])
+  );
   assume (M[Net#a][0] < 0) && (M[Net#a][1] > 0);
   assume (R[Net#d] + C[Net#d]) == AT#Div(R[Net#b] + 1, 2);
   assume (R[Net#c] + C[Net#c]) == AT#Div(R[Net#b], 2);
-  assume (forall i: int :: 
-    (0 <= i) && (i < (R[Net#b] + C[Net#b])) ==> (M[Net#b][i] == M[Net#a][i])
-  );
   assume (forall i: int :: 
     (0 <= i) && (i < R[Net#b]) && (AT#Mod(i, 2) == 0) ==> (M[Net#b][i] == M[Net#d][AT#Div(i, 2)])
   );
@@ -129,28 +129,28 @@ procedure Net#anon$3#Repeater#anon$0#4()
   C[Net#a] := C[Net#a] - 1;
   M[Net#b][R[Net#b] + C[Net#b]] := in#i;
   C[Net#b] := C[Net#b] + 1;
-  assert {:msg "  Sub-actor action at 3.3 might not preserve the channel invariant (generated)"} R[Net#a] == (R[Net#b] + C[Net#b]);
-  assert {:msg "  Sub-actor action at 3.3 might not preserve the channel invariant (generated)"} R[Net#d] == 0;
-  assert {:msg "  Sub-actor action at 3.3 might not preserve the channel invariant (generated)"} 0 <= C[Net#d];
-  assert {:msg "  Sub-actor action at 3.3 might not preserve the channel invariant (generated)"} 0 <= R[Net#d];
-  assert {:msg "  Sub-actor action at 3.3 might not preserve the channel invariant (generated)"} R[Net#c] == 0;
-  assert {:msg "  Sub-actor action at 3.3 might not preserve the channel invariant (generated)"} 0 <= C[Net#c];
-  assert {:msg "  Sub-actor action at 3.3 might not preserve the channel invariant (generated)"} 0 <= R[Net#c];
-  assert {:msg "  Sub-actor action at 3.3 might not preserve the channel invariant (generated)"} 0 <= C[Net#b];
-  assert {:msg "  Sub-actor action at 3.3 might not preserve the channel invariant (generated)"} 0 <= R[Net#b];
-  assert {:msg "  Sub-actor action at 3.3 might not preserve the channel invariant (generated)"} (R[Net#a] + C[Net#a]) == C#init[Net#a];
-  assert {:msg "  Sub-actor action at 3.3 might not preserve the channel invariant (generated)"} 0 <= C[Net#a];
-  assert {:msg "  Sub-actor action at 3.3 might not preserve the channel invariant (generated)"} 0 <= R[Net#a];
+  assert {:msg "  Sub-actor action at 3.3 might not preserve the channel invariant (generated #13)"} 0 <= R[Net#a];
+  assert {:msg "  Sub-actor action at 3.3 might not preserve the channel invariant (generated #14)"} 0 <= C[Net#a];
+  assert {:msg "  Sub-actor action at 3.3 might not preserve the channel invariant (generated #15)"} (R[Net#a] + C[Net#a]) == C#init[Net#a];
+  assert {:msg "  Sub-actor action at 3.3 might not preserve the channel invariant (generated #16)"} 0 <= R[Net#b];
+  assert {:msg "  Sub-actor action at 3.3 might not preserve the channel invariant (generated #17)"} 0 <= C[Net#b];
+  assert {:msg "  Sub-actor action at 3.3 might not preserve the channel invariant (generated #18)"} 0 <= R[Net#c];
+  assert {:msg "  Sub-actor action at 3.3 might not preserve the channel invariant (generated #19)"} 0 <= C[Net#c];
+  assert {:msg "  Sub-actor action at 3.3 might not preserve the channel invariant (generated #20)"} R[Net#c] == 0;
+  assert {:msg "  Sub-actor action at 3.3 might not preserve the channel invariant (generated #21)"} 0 <= R[Net#d];
+  assert {:msg "  Sub-actor action at 3.3 might not preserve the channel invariant (generated #22)"} 0 <= C[Net#d];
+  assert {:msg "  Sub-actor action at 3.3 might not preserve the channel invariant (generated #23)"} R[Net#d] == 0;
+  assert {:msg "  Sub-actor action at 3.3 might not preserve the channel invariant (generated #24)"} R[Net#a] == (R[Net#b] + C[Net#b]);
+  assert {:msg "  Sub-actor action at 3.3 might not preserve the channel invariant (generated #25)"} (forall idx: int :: 
+    (0 <= idx) && (idx < (R[Net#b] + C[Net#b])) ==> (M[Net#b][idx] == M[Net#a][idx])
+  );
   assert {:msg "  20.3: Sub-actor action at 3.3 might not preserve the channel invariant"} (M[Net#a][0] < 0) && (M[Net#a][1] > 0);
   assert {:msg "  21.3: Sub-actor action at 3.3 might not preserve the channel invariant"} (R[Net#d] + C[Net#d]) == AT#Div(R[Net#b] + 1, 2);
   assert {:msg "  22.3: Sub-actor action at 3.3 might not preserve the channel invariant"} (R[Net#c] + C[Net#c]) == AT#Div(R[Net#b], 2);
   assert {:msg "  23.3: Sub-actor action at 3.3 might not preserve the channel invariant"} (forall i: int :: 
-    (0 <= i) && (i < (R[Net#b] + C[Net#b])) ==> (M[Net#b][i] == M[Net#a][i])
-  );
-  assert {:msg "  24.3: Sub-actor action at 3.3 might not preserve the channel invariant"} (forall i: int :: 
     (0 <= i) && (i < R[Net#b]) && (AT#Mod(i, 2) == 0) ==> (M[Net#b][i] == M[Net#d][AT#Div(i, 2)])
   );
-  assert {:msg "  25.3: Sub-actor action at 3.3 might not preserve the channel invariant"} (forall i: int :: 
+  assert {:msg "  24.3: Sub-actor action at 3.3 might not preserve the channel invariant"} (forall i: int :: 
     (0 <= i) && (i < R[Net#b]) && (AT#Mod(i, 2) == 1) ==> (M[Net#b][i] == M[Net#c][AT#Div(i, 2)])
   );
 }
@@ -163,24 +163,24 @@ procedure Net#anon$3#Split#anon$1#5()
   assume C#init[Net#b] == 0;
   assume C#init[Net#c] == 0;
   assume C#init[Net#d] == 0;
-  assume R[Net#a] == (R[Net#b] + C[Net#b]);
-  assume R[Net#d] == 0;
-  assume 0 <= C[Net#d];
-  assume 0 <= R[Net#d];
-  assume R[Net#c] == 0;
-  assume 0 <= C[Net#c];
-  assume 0 <= R[Net#c];
-  assume 0 <= C[Net#b];
-  assume 0 <= R[Net#b];
-  assume (R[Net#a] + C[Net#a]) == C#init[Net#a];
-  assume 0 <= C[Net#a];
   assume 0 <= R[Net#a];
+  assume 0 <= C[Net#a];
+  assume (R[Net#a] + C[Net#a]) == C#init[Net#a];
+  assume 0 <= R[Net#b];
+  assume 0 <= C[Net#b];
+  assume 0 <= R[Net#c];
+  assume 0 <= C[Net#c];
+  assume R[Net#c] == 0;
+  assume 0 <= R[Net#d];
+  assume 0 <= C[Net#d];
+  assume R[Net#d] == 0;
+  assume R[Net#a] == (R[Net#b] + C[Net#b]);
+  assume (forall idx: int :: 
+    (0 <= idx) && (idx < (R[Net#b] + C[Net#b])) ==> (M[Net#b][idx] == M[Net#a][idx])
+  );
   assume (M[Net#a][0] < 0) && (M[Net#a][1] > 0);
   assume (R[Net#d] + C[Net#d]) == AT#Div(R[Net#b] + 1, 2);
   assume (R[Net#c] + C[Net#c]) == AT#Div(R[Net#b], 2);
-  assume (forall i: int :: 
-    (0 <= i) && (i < (R[Net#b] + C[Net#b])) ==> (M[Net#b][i] == M[Net#a][i])
-  );
   assume (forall i: int :: 
     (0 <= i) && (i < R[Net#b]) && (AT#Mod(i, 2) == 0) ==> (M[Net#b][i] == M[Net#d][AT#Div(i, 2)])
   );
@@ -195,28 +195,28 @@ procedure Net#anon$3#Split#anon$1#5()
   C[Net#b] := C[Net#b] - 1;
   M[Net#c][R[Net#c] + C[Net#c]] := in#i;
   C[Net#c] := C[Net#c] + 1;
-  assert {:msg "  Sub-actor action at 7.3 might not preserve the channel invariant (generated)"} R[Net#a] == (R[Net#b] + C[Net#b]);
-  assert {:msg "  Sub-actor action at 7.3 might not preserve the channel invariant (generated)"} R[Net#d] == 0;
-  assert {:msg "  Sub-actor action at 7.3 might not preserve the channel invariant (generated)"} 0 <= C[Net#d];
-  assert {:msg "  Sub-actor action at 7.3 might not preserve the channel invariant (generated)"} 0 <= R[Net#d];
-  assert {:msg "  Sub-actor action at 7.3 might not preserve the channel invariant (generated)"} R[Net#c] == 0;
-  assert {:msg "  Sub-actor action at 7.3 might not preserve the channel invariant (generated)"} 0 <= C[Net#c];
-  assert {:msg "  Sub-actor action at 7.3 might not preserve the channel invariant (generated)"} 0 <= R[Net#c];
-  assert {:msg "  Sub-actor action at 7.3 might not preserve the channel invariant (generated)"} 0 <= C[Net#b];
-  assert {:msg "  Sub-actor action at 7.3 might not preserve the channel invariant (generated)"} 0 <= R[Net#b];
-  assert {:msg "  Sub-actor action at 7.3 might not preserve the channel invariant (generated)"} (R[Net#a] + C[Net#a]) == C#init[Net#a];
-  assert {:msg "  Sub-actor action at 7.3 might not preserve the channel invariant (generated)"} 0 <= C[Net#a];
-  assert {:msg "  Sub-actor action at 7.3 might not preserve the channel invariant (generated)"} 0 <= R[Net#a];
+  assert {:msg "  Sub-actor action at 7.3 might not preserve the channel invariant (generated #26)"} 0 <= R[Net#a];
+  assert {:msg "  Sub-actor action at 7.3 might not preserve the channel invariant (generated #27)"} 0 <= C[Net#a];
+  assert {:msg "  Sub-actor action at 7.3 might not preserve the channel invariant (generated #28)"} (R[Net#a] + C[Net#a]) == C#init[Net#a];
+  assert {:msg "  Sub-actor action at 7.3 might not preserve the channel invariant (generated #29)"} 0 <= R[Net#b];
+  assert {:msg "  Sub-actor action at 7.3 might not preserve the channel invariant (generated #30)"} 0 <= C[Net#b];
+  assert {:msg "  Sub-actor action at 7.3 might not preserve the channel invariant (generated #31)"} 0 <= R[Net#c];
+  assert {:msg "  Sub-actor action at 7.3 might not preserve the channel invariant (generated #32)"} 0 <= C[Net#c];
+  assert {:msg "  Sub-actor action at 7.3 might not preserve the channel invariant (generated #33)"} R[Net#c] == 0;
+  assert {:msg "  Sub-actor action at 7.3 might not preserve the channel invariant (generated #34)"} 0 <= R[Net#d];
+  assert {:msg "  Sub-actor action at 7.3 might not preserve the channel invariant (generated #35)"} 0 <= C[Net#d];
+  assert {:msg "  Sub-actor action at 7.3 might not preserve the channel invariant (generated #36)"} R[Net#d] == 0;
+  assert {:msg "  Sub-actor action at 7.3 might not preserve the channel invariant (generated #37)"} R[Net#a] == (R[Net#b] + C[Net#b]);
+  assert {:msg "  Sub-actor action at 7.3 might not preserve the channel invariant (generated #38)"} (forall idx: int :: 
+    (0 <= idx) && (idx < (R[Net#b] + C[Net#b])) ==> (M[Net#b][idx] == M[Net#a][idx])
+  );
   assert {:msg "  20.3: Sub-actor action at 7.3 might not preserve the channel invariant"} (M[Net#a][0] < 0) && (M[Net#a][1] > 0);
   assert {:msg "  21.3: Sub-actor action at 7.3 might not preserve the channel invariant"} (R[Net#d] + C[Net#d]) == AT#Div(R[Net#b] + 1, 2);
   assert {:msg "  22.3: Sub-actor action at 7.3 might not preserve the channel invariant"} (R[Net#c] + C[Net#c]) == AT#Div(R[Net#b], 2);
   assert {:msg "  23.3: Sub-actor action at 7.3 might not preserve the channel invariant"} (forall i: int :: 
-    (0 <= i) && (i < (R[Net#b] + C[Net#b])) ==> (M[Net#b][i] == M[Net#a][i])
-  );
-  assert {:msg "  24.3: Sub-actor action at 7.3 might not preserve the channel invariant"} (forall i: int :: 
     (0 <= i) && (i < R[Net#b]) && (AT#Mod(i, 2) == 0) ==> (M[Net#b][i] == M[Net#d][AT#Div(i, 2)])
   );
-  assert {:msg "  25.3: Sub-actor action at 7.3 might not preserve the channel invariant"} (forall i: int :: 
+  assert {:msg "  24.3: Sub-actor action at 7.3 might not preserve the channel invariant"} (forall i: int :: 
     (0 <= i) && (i < R[Net#b]) && (AT#Mod(i, 2) == 1) ==> (M[Net#b][i] == M[Net#c][AT#Div(i, 2)])
   );
 }
@@ -229,24 +229,24 @@ procedure Net#anon$3#Split#anon$2#6()
   assume C#init[Net#b] == 0;
   assume C#init[Net#c] == 0;
   assume C#init[Net#d] == 0;
-  assume R[Net#a] == (R[Net#b] + C[Net#b]);
-  assume R[Net#d] == 0;
-  assume 0 <= C[Net#d];
-  assume 0 <= R[Net#d];
-  assume R[Net#c] == 0;
-  assume 0 <= C[Net#c];
-  assume 0 <= R[Net#c];
-  assume 0 <= C[Net#b];
-  assume 0 <= R[Net#b];
-  assume (R[Net#a] + C[Net#a]) == C#init[Net#a];
-  assume 0 <= C[Net#a];
   assume 0 <= R[Net#a];
+  assume 0 <= C[Net#a];
+  assume (R[Net#a] + C[Net#a]) == C#init[Net#a];
+  assume 0 <= R[Net#b];
+  assume 0 <= C[Net#b];
+  assume 0 <= R[Net#c];
+  assume 0 <= C[Net#c];
+  assume R[Net#c] == 0;
+  assume 0 <= R[Net#d];
+  assume 0 <= C[Net#d];
+  assume R[Net#d] == 0;
+  assume R[Net#a] == (R[Net#b] + C[Net#b]);
+  assume (forall idx: int :: 
+    (0 <= idx) && (idx < (R[Net#b] + C[Net#b])) ==> (M[Net#b][idx] == M[Net#a][idx])
+  );
   assume (M[Net#a][0] < 0) && (M[Net#a][1] > 0);
   assume (R[Net#d] + C[Net#d]) == AT#Div(R[Net#b] + 1, 2);
   assume (R[Net#c] + C[Net#c]) == AT#Div(R[Net#b], 2);
-  assume (forall i: int :: 
-    (0 <= i) && (i < (R[Net#b] + C[Net#b])) ==> (M[Net#b][i] == M[Net#a][i])
-  );
   assume (forall i: int :: 
     (0 <= i) && (i < R[Net#b]) && (AT#Mod(i, 2) == 0) ==> (M[Net#b][i] == M[Net#d][AT#Div(i, 2)])
   );
@@ -261,28 +261,28 @@ procedure Net#anon$3#Split#anon$2#6()
   C[Net#b] := C[Net#b] - 1;
   M[Net#d][R[Net#d] + C[Net#d]] := in#i;
   C[Net#d] := C[Net#d] + 1;
-  assert {:msg "  Sub-actor action at 10.3 might not preserve the channel invariant (generated)"} R[Net#a] == (R[Net#b] + C[Net#b]);
-  assert {:msg "  Sub-actor action at 10.3 might not preserve the channel invariant (generated)"} R[Net#d] == 0;
-  assert {:msg "  Sub-actor action at 10.3 might not preserve the channel invariant (generated)"} 0 <= C[Net#d];
-  assert {:msg "  Sub-actor action at 10.3 might not preserve the channel invariant (generated)"} 0 <= R[Net#d];
-  assert {:msg "  Sub-actor action at 10.3 might not preserve the channel invariant (generated)"} R[Net#c] == 0;
-  assert {:msg "  Sub-actor action at 10.3 might not preserve the channel invariant (generated)"} 0 <= C[Net#c];
-  assert {:msg "  Sub-actor action at 10.3 might not preserve the channel invariant (generated)"} 0 <= R[Net#c];
-  assert {:msg "  Sub-actor action at 10.3 might not preserve the channel invariant (generated)"} 0 <= C[Net#b];
-  assert {:msg "  Sub-actor action at 10.3 might not preserve the channel invariant (generated)"} 0 <= R[Net#b];
-  assert {:msg "  Sub-actor action at 10.3 might not preserve the channel invariant (generated)"} (R[Net#a] + C[Net#a]) == C#init[Net#a];
-  assert {:msg "  Sub-actor action at 10.3 might not preserve the channel invariant (generated)"} 0 <= C[Net#a];
-  assert {:msg "  Sub-actor action at 10.3 might not preserve the channel invariant (generated)"} 0 <= R[Net#a];
+  assert {:msg "  Sub-actor action at 10.3 might not preserve the channel invariant (generated #39)"} 0 <= R[Net#a];
+  assert {:msg "  Sub-actor action at 10.3 might not preserve the channel invariant (generated #40)"} 0 <= C[Net#a];
+  assert {:msg "  Sub-actor action at 10.3 might not preserve the channel invariant (generated #41)"} (R[Net#a] + C[Net#a]) == C#init[Net#a];
+  assert {:msg "  Sub-actor action at 10.3 might not preserve the channel invariant (generated #42)"} 0 <= R[Net#b];
+  assert {:msg "  Sub-actor action at 10.3 might not preserve the channel invariant (generated #43)"} 0 <= C[Net#b];
+  assert {:msg "  Sub-actor action at 10.3 might not preserve the channel invariant (generated #44)"} 0 <= R[Net#c];
+  assert {:msg "  Sub-actor action at 10.3 might not preserve the channel invariant (generated #45)"} 0 <= C[Net#c];
+  assert {:msg "  Sub-actor action at 10.3 might not preserve the channel invariant (generated #46)"} R[Net#c] == 0;
+  assert {:msg "  Sub-actor action at 10.3 might not preserve the channel invariant (generated #47)"} 0 <= R[Net#d];
+  assert {:msg "  Sub-actor action at 10.3 might not preserve the channel invariant (generated #48)"} 0 <= C[Net#d];
+  assert {:msg "  Sub-actor action at 10.3 might not preserve the channel invariant (generated #49)"} R[Net#d] == 0;
+  assert {:msg "  Sub-actor action at 10.3 might not preserve the channel invariant (generated #50)"} R[Net#a] == (R[Net#b] + C[Net#b]);
+  assert {:msg "  Sub-actor action at 10.3 might not preserve the channel invariant (generated #51)"} (forall idx: int :: 
+    (0 <= idx) && (idx < (R[Net#b] + C[Net#b])) ==> (M[Net#b][idx] == M[Net#a][idx])
+  );
   assert {:msg "  20.3: Sub-actor action at 10.3 might not preserve the channel invariant"} (M[Net#a][0] < 0) && (M[Net#a][1] > 0);
   assert {:msg "  21.3: Sub-actor action at 10.3 might not preserve the channel invariant"} (R[Net#d] + C[Net#d]) == AT#Div(R[Net#b] + 1, 2);
   assert {:msg "  22.3: Sub-actor action at 10.3 might not preserve the channel invariant"} (R[Net#c] + C[Net#c]) == AT#Div(R[Net#b], 2);
   assert {:msg "  23.3: Sub-actor action at 10.3 might not preserve the channel invariant"} (forall i: int :: 
-    (0 <= i) && (i < (R[Net#b] + C[Net#b])) ==> (M[Net#b][i] == M[Net#a][i])
-  );
-  assert {:msg "  24.3: Sub-actor action at 10.3 might not preserve the channel invariant"} (forall i: int :: 
     (0 <= i) && (i < R[Net#b]) && (AT#Mod(i, 2) == 0) ==> (M[Net#b][i] == M[Net#d][AT#Div(i, 2)])
   );
-  assert {:msg "  25.3: Sub-actor action at 10.3 might not preserve the channel invariant"} (forall i: int :: 
+  assert {:msg "  24.3: Sub-actor action at 10.3 might not preserve the channel invariant"} (forall i: int :: 
     (0 <= i) && (i < R[Net#b]) && (AT#Mod(i, 2) == 1) ==> (M[Net#b][i] == M[Net#c][AT#Div(i, 2)])
   );
 }
@@ -293,24 +293,24 @@ procedure Net#anon$3#exit#7()
   assume C#init[Net#b] == 0;
   assume C#init[Net#c] == 0;
   assume C#init[Net#d] == 0;
-  assume R[Net#a] == (R[Net#b] + C[Net#b]);
-  assume R[Net#d] == 0;
-  assume 0 <= C[Net#d];
-  assume 0 <= R[Net#d];
-  assume R[Net#c] == 0;
-  assume 0 <= C[Net#c];
-  assume 0 <= R[Net#c];
-  assume 0 <= C[Net#b];
-  assume 0 <= R[Net#b];
-  assume (R[Net#a] + C[Net#a]) == C#init[Net#a];
-  assume 0 <= C[Net#a];
   assume 0 <= R[Net#a];
+  assume 0 <= C[Net#a];
+  assume (R[Net#a] + C[Net#a]) == C#init[Net#a];
+  assume 0 <= R[Net#b];
+  assume 0 <= C[Net#b];
+  assume 0 <= R[Net#c];
+  assume 0 <= C[Net#c];
+  assume R[Net#c] == 0;
+  assume 0 <= R[Net#d];
+  assume 0 <= C[Net#d];
+  assume R[Net#d] == 0;
+  assume R[Net#a] == (R[Net#b] + C[Net#b]);
+  assume (forall idx: int :: 
+    (0 <= idx) && (idx < (R[Net#b] + C[Net#b])) ==> (M[Net#b][idx] == M[Net#a][idx])
+  );
   assume (M[Net#a][0] < 0) && (M[Net#a][1] > 0);
   assume (R[Net#d] + C[Net#d]) == AT#Div(R[Net#b] + 1, 2);
   assume (R[Net#c] + C[Net#c]) == AT#Div(R[Net#b], 2);
-  assume (forall i: int :: 
-    (0 <= i) && (i < (R[Net#b] + C[Net#b])) ==> (M[Net#b][i] == M[Net#a][i])
-  );
   assume (forall i: int :: 
     (0 <= i) && (i < R[Net#b]) && (AT#Mod(i, 2) == 0) ==> (M[Net#b][i] == M[Net#d][AT#Div(i, 2)])
   );
