tests/IIR.bpl
@@ -99,48 +99,51 @@ procedure iir#anon$5#entry#5()
   assume C#init == C;
   assume C[iir#f] == 1;
   assume M[iir#f][R[iir#f]] == (171 * M[iir#g][R[iir#g] - 1]);
-  assert {:msg "  Channel invariant might not hold on action entry (generated)"} R[iir#f] == (R[iir#c] + C[iir#c]);
-  assert {:msg "  Channel invariant might not hold on action entry (generated)"} R[iir#b] == (R[iir#c] + C[iir#c]);
-  assert {:msg "  Channel invariant might not hold on action entry (generated)"} R[iir#c] == (R[iir#g] + C[iir#g]);
-  assert {:msg "  Channel invariant might not hold on action entry (generated)"} R[iir#c] == (R[iir#d] + C[iir#d]);
-  assert {:msg "  Channel invariant might not hold on action entry (generated)"} R[iir#d] == (R[iir#e] + C[iir#e]);
-  assert {:msg "  Channel invariant might not hold on action entry (generated)"} R[iir#a] == (R[iir#b] + C[iir#b]);
-  assert {:msg "  Channel invariant might not hold on action entry (generated)"} R[iir#e] == ((R[iir#f] + C[iir#f]) - 1);
-  assert {:msg "  Channel invariant might not hold on action entry (generated)"} R[iir#g] == 0;
-  assert {:msg "  Channel invariant might not hold on action entry (generated)"} 0 <= C[iir#g];
-  assert {:msg "  Channel invariant might not hold on action entry (generated)"} 0 <= R[iir#g];
-  assert {:msg "  Channel invariant might not hold on action entry (generated)"} 0 <= C[iir#f];
-  assert {:msg "  Channel invariant might not hold on action entry (generated)"} 0 <= R[iir#f];
-  assert {:msg "  Channel invariant might not hold on action entry (generated)"} 0 <= C[iir#e];
-  assert {:msg "  Channel invariant might not hold on action entry (generated)"} 0 <= R[iir#e];
-  assert {:msg "  Channel invariant might not hold on action entry (generated)"} 0 <= C[iir#d];
-  assert {:msg "  Channel invariant might not hold on action entry (generated)"} 0 <= R[iir#d];
-  assert {:msg "  Channel invariant might not hold on action entry (generated)"} 0 <= C[iir#c];
-  assert {:msg "  Channel invariant might not hold on action entry (generated)"} 0 <= R[iir#c];
-  assert {:msg "  Channel invariant might not hold on action entry (generated)"} 0 <= C[iir#b];
-  assert {:msg "  Channel invariant might not hold on action entry (generated)"} 0 <= R[iir#b];
-  assert {:msg "  Channel invariant might not hold on action entry (generated)"} (R[iir#a] + C[iir#a]) == C#init[iir#a];
-  assert {:msg "  Channel invariant might not hold on action entry (generated)"} 0 <= C[iir#a];
-  assert {:msg "  Channel invariant might not hold on action entry (generated)"} 0 <= R[iir#a];
+  assert {:msg "  Channel invariant might not hold on action entry (generated #0 )"} (forall idx$: int :: 
+    (0 <= idx$) && (idx$ < (R[iir#c] + C[iir#c])) ==> (M[iir#c][idx$ - 0] == (M[iir#b][idx$ - 0] + M[iir#f][idx$ - 0]))
+  );
+  assert {:msg "  Channel invariant might not hold on action entry (generated #1 )"} R[iir#f] == (R[iir#c] + C[iir#c]);
+  assert {:msg "  Channel invariant might not hold on action entry (generated #2 )"} (forall idx$: int :: 
+    (0 <= idx$) && (idx$ < (R[iir#c] + C[iir#c])) ==> (M[iir#c][idx$ - 0] == (M[iir#b][idx$ - 0] + M[iir#f][idx$ - 0]))
+  );
+  assert {:msg "  Channel invariant might not hold on action entry (generated #3 )"} R[iir#b] == (R[iir#c] + C[iir#c]);
+  assert {:msg "  Channel invariant might not hold on action entry (generated #4 )"} (forall idx$: int :: 
+    (0 <= idx$) && (idx$ < (R[iir#g] + C[iir#g])) ==> (M[iir#g][idx$ - 0] == AT#RShift(M[iir#c][idx$ - 0], 8))
+  );
+  assert {:msg "  Channel invariant might not hold on action entry (generated #5 )"} R[iir#c] == (R[iir#g] + C[iir#g]);
+  assert {:msg "  Channel invariant might not hold on action entry (generated #6 )"} (forall idx$: int :: 
+    (0 <= idx$) && (idx$ < (R[iir#d] + C[iir#d])) ==> (M[iir#d][idx$ - 0] == AT#RShift(M[iir#c][idx$ - 0], 8))
+  );
+  assert {:msg "  Channel invariant might not hold on action entry (generated #7 )"} R[iir#c] == (R[iir#d] + C[iir#d]);
+  assert {:msg "  Channel invariant might not hold on action entry (generated #8 )"} (forall idx$: int :: 
+    (0 <= idx$) && (idx$ < (R[iir#e] + C[iir#e])) ==> (M[iir#e][idx$ - 0] == (171 * M[iir#d][idx$ - 0]))
+  );
+  assert {:msg "  Channel invariant might not hold on action entry (generated #9 )"} R[iir#d] == (R[iir#e] + C[iir#e]);
+  assert {:msg "  Channel invariant might not hold on action entry (generated #10 )"} (forall idx$: int :: 
+    (0 <= idx$) && (idx$ < (R[iir#b] + C[iir#b])) ==> (M[iir#b][idx$ - 0] == (85 * M[iir#a][idx$ - 0]))
+  );
+  assert {:msg "  Channel invariant might not hold on action entry (generated #11 )"} R[iir#a] == (R[iir#b] + C[iir#b]);
+  assert {:msg "  Channel invariant might not hold on action entry (generated #12 )"} (forall idx$: int :: 
+    (0 <= idx$) && (idx$ < ((R[iir#f] + C[iir#f]) - 1)) ==> (M[iir#f][(idx$ + 1) - 0] == M[iir#e][idx$ - 0])
+  );
+  assert {:msg "  Channel invariant might not hold on action entry (generated #13 )"} R[iir#e] == ((R[iir#f] + C[iir#f]) - 1);
+  assert {:msg "  Channel invariant might not hold on action entry (generated #14 )"} R[iir#g] == 0;
+  assert {:msg "  Channel invariant might not hold on action entry (generated #15 )"} 0 <= C[iir#g];
+  assert {:msg "  Channel invariant might not hold on action entry (generated #16 )"} 0 <= R[iir#g];
+  assert {:msg "  Channel invariant might not hold on action entry (generated #17 )"} 0 <= C[iir#f];
+  assert {:msg "  Channel invariant might not hold on action entry (generated #18 )"} 0 <= R[iir#f];
+  assert {:msg "  Channel invariant might not hold on action entry (generated #19 )"} 0 <= C[iir#e];
+  assert {:msg "  Channel invariant might not hold on action entry (generated #20 )"} 0 <= R[iir#e];
+  assert {:msg "  Channel invariant might not hold on action entry (generated #21 )"} 0 <= C[iir#d];
+  assert {:msg "  Channel invariant might not hold on action entry (generated #22 )"} 0 <= R[iir#d];
+  assert {:msg "  Channel invariant might not hold on action entry (generated #23 )"} 0 <= C[iir#c];
+  assert {:msg "  Channel invariant might not hold on action entry (generated #24 )"} 0 <= R[iir#c];
+  assert {:msg "  Channel invariant might not hold on action entry (generated #25 )"} 0 <= C[iir#b];
+  assert {:msg "  Channel invariant might not hold on action entry (generated #26 )"} 0 <= R[iir#b];
+  assert {:msg "  Channel invariant might not hold on action entry (generated #27 )"} (R[iir#a] + C[iir#a]) == C#init[iir#a];
+  assert {:msg "  Channel invariant might not hold on action entry (generated #28 )"} 0 <= C[iir#a];
+  assert {:msg "  Channel invariant might not hold on action entry (generated #29 )"} 0 <= R[iir#a];
   assert {:msg "  28.3: Channel invariant might not hold on action entry"} (171 * M[iir#g][-1]) == M[iir#f][0];
-  assert {:msg "  29.3: Channel invariant might not hold on action entry"} (forall i: int :: 
-    (0 <= i) && (i < (R[iir#b] + C[iir#b])) ==> (M[iir#b][i] == (85 * M[iir#a][i]))
-  );
-  assert {:msg "  30.3: Channel invariant might not hold on action entry"} (forall i: int :: 
-    (0 <= i) && (i < (R[iir#c] + C[iir#c])) ==> (M[iir#c][i] == (M[iir#b][i] + M[iir#f][i]))
-  );
-  assert {:msg "  31.3: Channel invariant might not hold on action entry"} (forall i: int :: 
-    (0 <= i) && (i < (R[iir#d] + C[iir#d])) ==> (M[iir#d][i] == AT#RShift(M[iir#c][i], 8))
-  );
-  assert {:msg "  32.3: Channel invariant might not hold on action entry"} (forall i: int :: 
-    (0 <= i) && (i < (R[iir#g] + C[iir#g])) ==> (M[iir#g][i] == AT#RShift(M[iir#c][i], 8))
-  );
-  assert {:msg "  33.3: Channel invariant might not hold on action entry"} (forall i: int :: 
-    (0 <= i) && (i < (R[iir#e] + C[iir#e])) ==> (M[iir#e][i] == (171 * M[iir#d][i]))
-  );
-  assert {:msg "  34.3: Channel invariant might not hold on action entry"} (forall i: int :: 
-    (1 <= i) && (i < (R[iir#f] + C[iir#f])) ==> (M[iir#f][i] == M[iir#e][i - 1])
-  );
 }
 procedure iir#anon$5#delay#anon$2#6()
   modifies C, R, M, St;
@@ -155,12 +158,33 @@ procedure iir#anon$5#delay#anon$2#6()
   assume C#init[iir#d] == 0;
   assume C#init[iir#e] == 0;
   assume C#init[iir#g] == 0;
+  assume (forall idx$: int :: 
+    (0 <= idx$) && (idx$ < (R[iir#c] + C[iir#c])) ==> (M[iir#c][idx$ - 0] == (M[iir#b][idx$ - 0] + M[iir#f][idx$ - 0]))
+  );
   assume R[iir#f] == (R[iir#c] + C[iir#c]);
+  assume (forall idx$: int :: 
+    (0 <= idx$) && (idx$ < (R[iir#c] + C[iir#c])) ==> (M[iir#c][idx$ - 0] == (M[iir#b][idx$ - 0] + M[iir#f][idx$ - 0]))
+  );
   assume R[iir#b] == (R[iir#c] + C[iir#c]);
+  assume (forall idx$: int :: 
+    (0 <= idx$) && (idx$ < (R[iir#g] + C[iir#g])) ==> (M[iir#g][idx$ - 0] == AT#RShift(M[iir#c][idx$ - 0], 8))
+  );
   assume R[iir#c] == (R[iir#g] + C[iir#g]);
+  assume (forall idx$: int :: 
+    (0 <= idx$) && (idx$ < (R[iir#d] + C[iir#d])) ==> (M[iir#d][idx$ - 0] == AT#RShift(M[iir#c][idx$ - 0], 8))
+  );
   assume R[iir#c] == (R[iir#d] + C[iir#d]);
+  assume (forall idx$: int :: 
+    (0 <= idx$) && (idx$ < (R[iir#e] + C[iir#e])) ==> (M[iir#e][idx$ - 0] == (171 * M[iir#d][idx$ - 0]))
+  );
   assume R[iir#d] == (R[iir#e] + C[iir#e]);
+  assume (forall idx$: int :: 
+    (0 <= idx$) && (idx$ < (R[iir#b] + C[iir#b])) ==> (M[iir#b][idx$ - 0] == (85 * M[iir#a][idx$ - 0]))
+  );
   assume R[iir#a] == (R[iir#b] + C[iir#b]);
+  assume (forall idx$: int :: 
+    (0 <= idx$) && (idx$ < ((R[iir#f] + C[iir#f]) - 1)) ==> (M[iir#f][(idx$ + 1) - 0] == M[iir#e][idx$ - 0])
+  );
   assume R[iir#e] == ((R[iir#f] + C[iir#f]) - 1);
   assume R[iir#g] == 0;
   assume 0 <= C[iir#g];
@@ -179,24 +203,6 @@ procedure iir#anon$5#delay#anon$2#6()
   assume 0 <= C[iir#a];
   assume 0 <= R[iir#a];
   assume (171 * M[iir#g][-1]) == M[iir#f][0];
-  assume (forall i: int :: 
-    (0 <= i) && (i < (R[iir#b] + C[iir#b])) ==> (M[iir#b][i] == (85 * M[iir#a][i]))
-  );
-  assume (forall i: int :: 
-    (0 <= i) && (i < (R[iir#c] + C[iir#c])) ==> (M[iir#c][i] == (M[iir#b][i] + M[iir#f][i]))
-  );
-  assume (forall i: int :: 
-    (0 <= i) && (i < (R[iir#d] + C[iir#d])) ==> (M[iir#d][i] == AT#RShift(M[iir#c][i], 8))
-  );
-  assume (forall i: int :: 
-    (0 <= i) && (i < (R[iir#g] + C[iir#g])) ==> (M[iir#g][i] == AT#RShift(M[iir#c][i], 8))
-  );
-  assume (forall i: int :: 
-    (0 <= i) && (i < (R[iir#e] + C[iir#e])) ==> (M[iir#e][i] == (171 * M[iir#d][i]))
-  );
-  assume (forall i: int :: 
-    (1 <= i) && (i < (R[iir#f] + C[iir#f])) ==> (M[iir#f][i] == M[iir#e][i - 1])
-  );
   assume true;
   assume 1 <= C[iir#e];
   in#i := M[iir#e][R[iir#e]];
@@ -204,48 +210,51 @@ procedure iir#anon$5#delay#anon$2#6()
   C[iir#e] := C[iir#e] - 1;
   M[iir#f][R[iir#f] + C[iir#f]] := in#i;
   C[iir#f] := C[iir#f] + 1;
-  assert {:msg "  Sub-actor action at 9.3 might not preserve the channel invariant (generated)"} R[iir#f] == (R[iir#c] + C[iir#c]);
-  assert {:msg "  Sub-actor action at 9.3 might not preserve the channel invariant (generated)"} R[iir#b] == (R[iir#c] + C[iir#c]);
-  assert {:msg "  Sub-actor action at 9.3 might not preserve the channel invariant (generated)"} R[iir#c] == (R[iir#g] + C[iir#g]);
-  assert {:msg "  Sub-actor action at 9.3 might not preserve the channel invariant (generated)"} R[iir#c] == (R[iir#d] + C[iir#d]);
-  assert {:msg "  Sub-actor action at 9.3 might not preserve the channel invariant (generated)"} R[iir#d] == (R[iir#e] + C[iir#e]);
-  assert {:msg "  Sub-actor action at 9.3 might not preserve the channel invariant (generated)"} R[iir#a] == (R[iir#b] + C[iir#b]);
-  assert {:msg "  Sub-actor action at 9.3 might not preserve the channel invariant (generated)"} R[iir#e] == ((R[iir#f] + C[iir#f]) - 1);
-  assert {:msg "  Sub-actor action at 9.3 might not preserve the channel invariant (generated)"} R[iir#g] == 0;
-  assert {:msg "  Sub-actor action at 9.3 might not preserve the channel invariant (generated)"} 0 <= C[iir#g];
-  assert {:msg "  Sub-actor action at 9.3 might not preserve the channel invariant (generated)"} 0 <= R[iir#g];
-  assert {:msg "  Sub-actor action at 9.3 might not preserve the channel invariant (generated)"} 0 <= C[iir#f];
-  assert {:msg "  Sub-actor action at 9.3 might not preserve the channel invariant (generated)"} 0 <= R[iir#f];
-  assert {:msg "  Sub-actor action at 9.3 might not preserve the channel invariant (generated)"} 0 <= C[iir#e];
-  assert {:msg "  Sub-actor action at 9.3 might not preserve the channel invariant (generated)"} 0 <= R[iir#e];
-  assert {:msg "  Sub-actor action at 9.3 might not preserve the channel invariant (generated)"} 0 <= C[iir#d];
-  assert {:msg "  Sub-actor action at 9.3 might not preserve the channel invariant (generated)"} 0 <= R[iir#d];
-  assert {:msg "  Sub-actor action at 9.3 might not preserve the channel invariant (generated)"} 0 <= C[iir#c];
-  assert {:msg "  Sub-actor action at 9.3 might not preserve the channel invariant (generated)"} 0 <= R[iir#c];
-  assert {:msg "  Sub-actor action at 9.3 might not preserve the channel invariant (generated)"} 0 <= C[iir#b];
-  assert {:msg "  Sub-actor action at 9.3 might not preserve the channel invariant (generated)"} 0 <= R[iir#b];
-  assert {:msg "  Sub-actor action at 9.3 might not preserve the channel invariant (generated)"} (R[iir#a] + C[iir#a]) == C#init[iir#a];
-  assert {:msg "  Sub-actor action at 9.3 might not preserve the channel invariant (generated)"} 0 <= C[iir#a];
-  assert {:msg "  Sub-actor action at 9.3 might not preserve the channel invariant (generated)"} 0 <= R[iir#a];
+  assert {:msg "  Sub-actor action at 9.3 might not preserve the channel invariant (generated #30)"} (forall idx$: int :: 
+    (0 <= idx$) && (idx$ < (R[iir#c] + C[iir#c])) ==> (M[iir#c][idx$ - 0] == (M[iir#b][idx$ - 0] + M[iir#f][idx$ - 0]))
+  );
+  assert {:msg "  Sub-actor action at 9.3 might not preserve the channel invariant (generated #31)"} R[iir#f] == (R[iir#c] + C[iir#c]);
+  assert {:msg "  Sub-actor action at 9.3 might not preserve the channel invariant (generated #32)"} (forall idx$: int :: 
+    (0 <= idx$) && (idx$ < (R[iir#c] + C[iir#c])) ==> (M[iir#c][idx$ - 0] == (M[iir#b][idx$ - 0] + M[iir#f][idx$ - 0]))
+  );
+  assert {:msg "  Sub-actor action at 9.3 might not preserve the channel invariant (generated #33)"} R[iir#b] == (R[iir#c] + C[iir#c]);
+  assert {:msg "  Sub-actor action at 9.3 might not preserve the channel invariant (generated #34)"} (forall idx$: int :: 
+    (0 <= idx$) && (idx$ < (R[iir#g] + C[iir#g])) ==> (M[iir#g][idx$ - 0] == AT#RShift(M[iir#c][idx$ - 0], 8))
+  );
+  assert {:msg "  Sub-actor action at 9.3 might not preserve the channel invariant (generated #35)"} R[iir#c] == (R[iir#g] + C[iir#g]);
+  assert {:msg "  Sub-actor action at 9.3 might not preserve the channel invariant (generated #36)"} (forall idx$: int :: 
+    (0 <= idx$) && (idx$ < (R[iir#d] + C[iir#d])) ==> (M[iir#d][idx$ - 0] == AT#RShift(M[iir#c][idx$ - 0], 8))
+  );
+  assert {:msg "  Sub-actor action at 9.3 might not preserve the channel invariant (generated #37)"} R[iir#c] == (R[iir#d] + C[iir#d]);
+  assert {:msg "  Sub-actor action at 9.3 might not preserve the channel invariant (generated #38)"} (forall idx$: int :: 
+    (0 <= idx$) && (idx$ < (R[iir#e] + C[iir#e])) ==> (M[iir#e][idx$ - 0] == (171 * M[iir#d][idx$ - 0]))
+  );
+  assert {:msg "  Sub-actor action at 9.3 might not preserve the channel invariant (generated #39)"} R[iir#d] == (R[iir#e] + C[iir#e]);
+  assert {:msg "  Sub-actor action at 9.3 might not preserve the channel invariant (generated #40)"} (forall idx$: int :: 
+    (0 <= idx$) && (idx$ < (R[iir#b] + C[iir#b])) ==> (M[iir#b][idx$ - 0] == (85 * M[iir#a][idx$ - 0]))
+  );
+  assert {:msg "  Sub-actor action at 9.3 might not preserve the channel invariant (generated #41)"} R[iir#a] == (R[iir#b] + C[iir#b]);
+  assert {:msg "  Sub-actor action at 9.3 might not preserve the channel invariant (generated #42)"} (forall idx$: int :: 
+    (0 <= idx$) && (idx$ < ((R[iir#f] + C[iir#f]) - 1)) ==> (M[iir#f][(idx$ + 1) - 0] == M[iir#e][idx$ - 0])
+  );
+  assert {:msg "  Sub-actor action at 9.3 might not preserve the channel invariant (generated #43)"} R[iir#e] == ((R[iir#f] + C[iir#f]) - 1);
+  assert {:msg "  Sub-actor action at 9.3 might not preserve the channel invariant (generated #44)"} R[iir#g] == 0;
+  assert {:msg "  Sub-actor action at 9.3 might not preserve the channel invariant (generated #45)"} 0 <= C[iir#g];
+  assert {:msg "  Sub-actor action at 9.3 might not preserve the channel invariant (generated #46)"} 0 <= R[iir#g];
+  assert {:msg "  Sub-actor action at 9.3 might not preserve the channel invariant (generated #47)"} 0 <= C[iir#f];
+  assert {:msg "  Sub-actor action at 9.3 might not preserve the channel invariant (generated #48)"} 0 <= R[iir#f];
+  assert {:msg "  Sub-actor action at 9.3 might not preserve the channel invariant (generated #49)"} 0 <= C[iir#e];
+  assert {:msg "  Sub-actor action at 9.3 might not preserve the channel invariant (generated #50)"} 0 <= R[iir#e];
+  assert {:msg "  Sub-actor action at 9.3 might not preserve the channel invariant (generated #51)"} 0 <= C[iir#d];
+  assert {:msg "  Sub-actor action at 9.3 might not preserve the channel invariant (generated #52)"} 0 <= R[iir#d];
+  assert {:msg "  Sub-actor action at 9.3 might not preserve the channel invariant (generated #53)"} 0 <= C[iir#c];
+  assert {:msg "  Sub-actor action at 9.3 might not preserve the channel invariant (generated #54)"} 0 <= R[iir#c];
+  assert {:msg "  Sub-actor action at 9.3 might not preserve the channel invariant (generated #55)"} 0 <= C[iir#b];
+  assert {:msg "  Sub-actor action at 9.3 might not preserve the channel invariant (generated #56)"} 0 <= R[iir#b];
+  assert {:msg "  Sub-actor action at 9.3 might not preserve the channel invariant (generated #57)"} (R[iir#a] + C[iir#a]) == C#init[iir#a];
+  assert {:msg "  Sub-actor action at 9.3 might not preserve the channel invariant (generated #58)"} 0 <= C[iir#a];
+  assert {:msg "  Sub-actor action at 9.3 might not preserve the channel invariant (generated #59)"} 0 <= R[iir#a];
   assert {:msg "  28.3: Sub-actor action at 9.3 might not preserve the channel invariant"} (171 * M[iir#g][-1]) == M[iir#f][0];
-  assert {:msg "  29.3: Sub-actor action at 9.3 might not preserve the channel invariant"} (forall i: int :: 
-    (0 <= i) && (i < (R[iir#b] + C[iir#b])) ==> (M[iir#b][i] == (85 * M[iir#a][i]))
-  );
-  assert {:msg "  30.3: Sub-actor action at 9.3 might not preserve the channel invariant"} (forall i: int :: 
-    (0 <= i) && (i < (R[iir#c] + C[iir#c])) ==> (M[iir#c][i] == (M[iir#b][i] + M[iir#f][i]))
-  );
-  assert {:msg "  31.3: Sub-actor action at 9.3 might not preserve the channel invariant"} (forall i: int :: 
-    (0 <= i) && (i < (R[iir#d] + C[iir#d])) ==> (M[iir#d][i] == AT#RShift(M[iir#c][i], 8))
-  );
-  assert {:msg "  32.3: Sub-actor action at 9.3 might not preserve the channel invariant"} (forall i: int :: 
-    (0 <= i) && (i < (R[iir#g] + C[iir#g])) ==> (M[iir#g][i] == AT#RShift(M[iir#c][i], 8))
-  );
-  assert {:msg "  33.3: Sub-actor action at 9.3 might not preserve the channel invariant"} (forall i: int :: 
-    (0 <= i) && (i < (R[iir#e] + C[iir#e])) ==> (M[iir#e][i] == (171 * M[iir#d][i]))
-  );
-  assert {:msg "  34.3: Sub-actor action at 9.3 might not preserve the channel invariant"} (forall i: int :: 
-    (1 <= i) && (i < (R[iir#f] + C[iir#f])) ==> (M[iir#f][i] == M[iir#e][i - 1])
-  );
 }
 procedure iir#anon$5#mulc#anon$3#7()
   modifies C, R, M, St;
@@ -260,12 +269,33 @@ procedure iir#anon$5#mulc#anon$3#7()
   assume C#init[iir#d] == 0;
   assume C#init[iir#e] == 0;
   assume C#init[iir#g] == 0;
+  assume (forall idx$: int :: 
+    (0 <= idx$) && (idx$ < (R[iir#c] + C[iir#c])) ==> (M[iir#c][idx$ - 0] == (M[iir#b][idx$ - 0] + M[iir#f][idx$ - 0]))
+  );
   assume R[iir#f] == (R[iir#c] + C[iir#c]);
+  assume (forall idx$: int :: 
+    (0 <= idx$) && (idx$ < (R[iir#c] + C[iir#c])) ==> (M[iir#c][idx$ - 0] == (M[iir#b][idx$ - 0] + M[iir#f][idx$ - 0]))
+  );
   assume R[iir#b] == (R[iir#c] + C[iir#c]);
+  assume (forall idx$: int :: 
+    (0 <= idx$) && (idx$ < (R[iir#g] + C[iir#g])) ==> (M[iir#g][idx$ - 0] == AT#RShift(M[iir#c][idx$ - 0], 8))
+  );
   assume R[iir#c] == (R[iir#g] + C[iir#g]);
+  assume (forall idx$: int :: 
+    (0 <= idx$) && (idx$ < (R[iir#d] + C[iir#d])) ==> (M[iir#d][idx$ - 0] == AT#RShift(M[iir#c][idx$ - 0], 8))
+  );
   assume R[iir#c] == (R[iir#d] + C[iir#d]);
+  assume (forall idx$: int :: 
+    (0 <= idx$) && (idx$ < (R[iir#e] + C[iir#e])) ==> (M[iir#e][idx$ - 0] == (171 * M[iir#d][idx$ - 0]))
+  );
   assume R[iir#d] == (R[iir#e] + C[iir#e]);
+  assume (forall idx$: int :: 
+    (0 <= idx$) && (idx$ < (R[iir#b] + C[iir#b])) ==> (M[iir#b][idx$ - 0] == (85 * M[iir#a][idx$ - 0]))
+  );
   assume R[iir#a] == (R[iir#b] + C[iir#b]);
+  assume (forall idx$: int :: 
+    (0 <= idx$) && (idx$ < ((R[iir#f] + C[iir#f]) - 1)) ==> (M[iir#f][(idx$ + 1) - 0] == M[iir#e][idx$ - 0])
+  );
   assume R[iir#e] == ((R[iir#f] + C[iir#f]) - 1);
   assume R[iir#g] == 0;
   assume 0 <= C[iir#g];
@@ -284,24 +314,6 @@ procedure iir#anon$5#mulc#anon$3#7()
   assume 0 <= C[iir#a];
   assume 0 <= R[iir#a];
   assume (171 * M[iir#g][-1]) == M[iir#f][0];
-  assume (forall i: int :: 
-    (0 <= i) && (i < (R[iir#b] + C[iir#b])) ==> (M[iir#b][i] == (85 * M[iir#a][i]))
-  );
-  assume (forall i: int :: 
-    (0 <= i) && (i < (R[iir#c] + C[iir#c])) ==> (M[iir#c][i] == (M[iir#b][i] + M[iir#f][i]))
-  );
-  assume (forall i: int :: 
-    (0 <= i) && (i < (R[iir#d] + C[iir#d])) ==> (M[iir#d][i] == AT#RShift(M[iir#c][i], 8))
-  );
-  assume (forall i: int :: 
-    (0 <= i) && (i < (R[iir#g] + C[iir#g])) ==> (M[iir#g][i] == AT#RShift(M[iir#c][i], 8))
-  );
-  assume (forall i: int :: 
-    (0 <= i) && (i < (R[iir#e] + C[iir#e])) ==> (M[iir#e][i] == (171 * M[iir#d][i]))
-  );
-  assume (forall i: int :: 
-    (1 <= i) && (i < (R[iir#f] + C[iir#f])) ==> (M[iir#f][i] == M[iir#e][i - 1])
-  );
   assume true;
   assume 1 <= C[iir#a];
   in#i := M[iir#a][R[iir#a]];
@@ -309,48 +321,51 @@ procedure iir#anon$5#mulc#anon$3#7()
   C[iir#a] := C[iir#a] - 1;
   M[iir#b][R[iir#b] + C[iir#b]] := ActorParam#c * in#i;
   C[iir#b] := C[iir#b] + 1;
-  assert {:msg "  Sub-actor action at 14.3 might not preserve the channel invariant (generated)"} R[iir#f] == (R[iir#c] + C[iir#c]);
-  assert {:msg "  Sub-actor action at 14.3 might not preserve the channel invariant (generated)"} R[iir#b] == (R[iir#c] + C[iir#c]);
-  assert {:msg "  Sub-actor action at 14.3 might not preserve the channel invariant (generated)"} R[iir#c] == (R[iir#g] + C[iir#g]);
-  assert {:msg "  Sub-actor action at 14.3 might not preserve the channel invariant (generated)"} R[iir#c] == (R[iir#d] + C[iir#d]);
-  assert {:msg "  Sub-actor action at 14.3 might not preserve the channel invariant (generated)"} R[iir#d] == (R[iir#e] + C[iir#e]);
-  assert {:msg "  Sub-actor action at 14.3 might not preserve the channel invariant (generated)"} R[iir#a] == (R[iir#b] + C[iir#b]);
-  assert {:msg "  Sub-actor action at 14.3 might not preserve the channel invariant (generated)"} R[iir#e] == ((R[iir#f] + C[iir#f]) - 1);
-  assert {:msg "  Sub-actor action at 14.3 might not preserve the channel invariant (generated)"} R[iir#g] == 0;
-  assert {:msg "  Sub-actor action at 14.3 might not preserve the channel invariant (generated)"} 0 <= C[iir#g];
-  assert {:msg "  Sub-actor action at 14.3 might not preserve the channel invariant (generated)"} 0 <= R[iir#g];
-  assert {:msg "  Sub-actor action at 14.3 might not preserve the channel invariant (generated)"} 0 <= C[iir#f];
-  assert {:msg "  Sub-actor action at 14.3 might not preserve the channel invariant (generated)"} 0 <= R[iir#f];
-  assert {:msg "  Sub-actor action at 14.3 might not preserve the channel invariant (generated)"} 0 <= C[iir#e];
-  assert {:msg "  Sub-actor action at 14.3 might not preserve the channel invariant (generated)"} 0 <= R[iir#e];
-  assert {:msg "  Sub-actor action at 14.3 might not preserve the channel invariant (generated)"} 0 <= C[iir#d];
-  assert {:msg "  Sub-actor action at 14.3 might not preserve the channel invariant (generated)"} 0 <= R[iir#d];
-  assert {:msg "  Sub-actor action at 14.3 might not preserve the channel invariant (generated)"} 0 <= C[iir#c];
-  assert {:msg "  Sub-actor action at 14.3 might not preserve the channel invariant (generated)"} 0 <= R[iir#c];
-  assert {:msg "  Sub-actor action at 14.3 might not preserve the channel invariant (generated)"} 0 <= C[iir#b];
-  assert {:msg "  Sub-actor action at 14.3 might not preserve the channel invariant (generated)"} 0 <= R[iir#b];
-  assert {:msg "  Sub-actor action at 14.3 might not preserve the channel invariant (generated)"} (R[iir#a] + C[iir#a]) == C#init[iir#a];
-  assert {:msg "  Sub-actor action at 14.3 might not preserve the channel invariant (generated)"} 0 <= C[iir#a];
-  assert {:msg "  Sub-actor action at 14.3 might not preserve the channel invariant (generated)"} 0 <= R[iir#a];
+  assert {:msg "  Sub-actor action at 14.3 might not preserve the channel invariant (generated #60)"} (forall idx$: int :: 
+    (0 <= idx$) && (idx$ < (R[iir#c] + C[iir#c])) ==> (M[iir#c][idx$ - 0] == (M[iir#b][idx$ - 0] + M[iir#f][idx$ - 0]))
+  );
+  assert {:msg "  Sub-actor action at 14.3 might not preserve the channel invariant (generated #61)"} R[iir#f] == (R[iir#c] + C[iir#c]);
+  assert {:msg "  Sub-actor action at 14.3 might not preserve the channel invariant (generated #62)"} (forall idx$: int :: 
+    (0 <= idx$) && (idx$ < (R[iir#c] + C[iir#c])) ==> (M[iir#c][idx$ - 0] == (M[iir#b][idx$ - 0] + M[iir#f][idx$ - 0]))
+  );
+  assert {:msg "  Sub-actor action at 14.3 might not preserve the channel invariant (generated #63)"} R[iir#b] == (R[iir#c] + C[iir#c]);
+  assert {:msg "  Sub-actor action at 14.3 might not preserve the channel invariant (generated #64)"} (forall idx$: int :: 
+    (0 <= idx$) && (idx$ < (R[iir#g] + C[iir#g])) ==> (M[iir#g][idx$ - 0] == AT#RShift(M[iir#c][idx$ - 0], 8))
+  );
+  assert {:msg "  Sub-actor action at 14.3 might not preserve the channel invariant (generated #65)"} R[iir#c] == (R[iir#g] + C[iir#g]);
+  assert {:msg "  Sub-actor action at 14.3 might not preserve the channel invariant (generated #66)"} (forall idx$: int :: 
+    (0 <= idx$) && (idx$ < (R[iir#d] + C[iir#d])) ==> (M[iir#d][idx$ - 0] == AT#RShift(M[iir#c][idx$ - 0], 8))
+  );
+  assert {:msg "  Sub-actor action at 14.3 might not preserve the channel invariant (generated #67)"} R[iir#c] == (R[iir#d] + C[iir#d]);
+  assert {:msg "  Sub-actor action at 14.3 might not preserve the channel invariant (generated #68)"} (forall idx$: int :: 
+    (0 <= idx$) && (idx$ < (R[iir#e] + C[iir#e])) ==> (M[iir#e][idx$ - 0] == (171 * M[iir#d][idx$ - 0]))
+  );
+  assert {:msg "  Sub-actor action at 14.3 might not preserve the channel invariant (generated #69)"} R[iir#d] == (R[iir#e] + C[iir#e]);
+  assert {:msg "  Sub-actor action at 14.3 might not preserve the channel invariant (generated #70)"} (forall idx$: int :: 
+    (0 <= idx$) && (idx$ < (R[iir#b] + C[iir#b])) ==> (M[iir#b][idx$ - 0] == (85 * M[iir#a][idx$ - 0]))
+  );
+  assert {:msg "  Sub-actor action at 14.3 might not preserve the channel invariant (generated #71)"} R[iir#a] == (R[iir#b] + C[iir#b]);
+  assert {:msg "  Sub-actor action at 14.3 might not preserve the channel invariant (generated #72)"} (forall idx$: int :: 
+    (0 <= idx$) && (idx$ < ((R[iir#f] + C[iir#f]) - 1)) ==> (M[iir#f][(idx$ + 1) - 0] == M[iir#e][idx$ - 0])
+  );
+  assert {:msg "  Sub-actor action at 14.3 might not preserve the channel invariant (generated #73)"} R[iir#e] == ((R[iir#f] + C[iir#f]) - 1);
+  assert {:msg "  Sub-actor action at 14.3 might not preserve the channel invariant (generated #74)"} R[iir#g] == 0;
+  assert {:msg "  Sub-actor action at 14.3 might not preserve the channel invariant (generated #75)"} 0 <= C[iir#g];
+  assert {:msg "  Sub-actor action at 14.3 might not preserve the channel invariant (generated #76)"} 0 <= R[iir#g];
+  assert {:msg "  Sub-actor action at 14.3 might not preserve the channel invariant (generated #77)"} 0 <= C[iir#f];
+  assert {:msg "  Sub-actor action at 14.3 might not preserve the channel invariant (generated #78)"} 0 <= R[iir#f];
+  assert {:msg "  Sub-actor action at 14.3 might not preserve the channel invariant (generated #79)"} 0 <= C[iir#e];
+  assert {:msg "  Sub-actor action at 14.3 might not preserve the channel invariant (generated #80)"} 0 <= R[iir#e];
+  assert {:msg "  Sub-actor action at 14.3 might not preserve the channel invariant (generated #81)"} 0 <= C[iir#d];
+  assert {:msg "  Sub-actor action at 14.3 might not preserve the channel invariant (generated #82)"} 0 <= R[iir#d];
+  assert {:msg "  Sub-actor action at 14.3 might not preserve the channel invariant (generated #83)"} 0 <= C[iir#c];
+  assert {:msg "  Sub-actor action at 14.3 might not preserve the channel invariant (generated #84)"} 0 <= R[iir#c];
+  assert {:msg "  Sub-actor action at 14.3 might not preserve the channel invariant (generated #85)"} 0 <= C[iir#b];
+  assert {:msg "  Sub-actor action at 14.3 might not preserve the channel invariant (generated #86)"} 0 <= R[iir#b];
+  assert {:msg "  Sub-actor action at 14.3 might not preserve the channel invariant (generated #87)"} (R[iir#a] + C[iir#a]) == C#init[iir#a];
+  assert {:msg "  Sub-actor action at 14.3 might not preserve the channel invariant (generated #88)"} 0 <= C[iir#a];
+  assert {:msg "  Sub-actor action at 14.3 might not preserve the channel invariant (generated #89)"} 0 <= R[iir#a];
   assert {:msg "  28.3: Sub-actor action at 14.3 might not preserve the channel invariant"} (171 * M[iir#g][-1]) == M[iir#f][0];
-  assert {:msg "  29.3: Sub-actor action at 14.3 might not preserve the channel invariant"} (forall i: int :: 
-    (0 <= i) && (i < (R[iir#b] + C[iir#b])) ==> (M[iir#b][i] == (85 * M[iir#a][i]))
-  );
-  assert {:msg "  30.3: Sub-actor action at 14.3 might not preserve the channel invariant"} (forall i: int :: 
-    (0 <= i) && (i < (R[iir#c] + C[iir#c])) ==> (M[iir#c][i] == (M[iir#b][i] + M[iir#f][i]))
-  );
-  assert {:msg "  31.3: Sub-actor action at 14.3 might not preserve the channel invariant"} (forall i: int :: 
-    (0 <= i) && (i < (R[iir#d] + C[iir#d])) ==> (M[iir#d][i] == AT#RShift(M[iir#c][i], 8))
-  );
-  assert {:msg "  32.3: Sub-actor action at 14.3 might not preserve the channel invariant"} (forall i: int :: 
-    (0 <= i) && (i < (R[iir#g] + C[iir#g])) ==> (M[iir#g][i] == AT#RShift(M[iir#c][i], 8))
-  );
-  assert {:msg "  33.3: Sub-actor action at 14.3 might not preserve the channel invariant"} (forall i: int :: 
-    (0 <= i) && (i < (R[iir#e] + C[iir#e])) ==> (M[iir#e][i] == (171 * M[iir#d][i]))
-  );
-  assert {:msg "  34.3: Sub-actor action at 14.3 might not preserve the channel invariant"} (forall i: int :: 
-    (1 <= i) && (i < (R[iir#f] + C[iir#f])) ==> (M[iir#f][i] == M[iir#e][i - 1])
-  );
 }
 procedure iir#anon$5#mulc#anon$3#8()
   modifies C, R, M, St;
@@ -365,12 +380,33 @@ procedure iir#anon$5#mulc#anon$3#8()
   assume C#init[iir#d] == 0;
   assume C#init[iir#e] == 0;
   assume C#init[iir#g] == 0;
+  assume (forall idx$: int :: 
+    (0 <= idx$) && (idx$ < (R[iir#c] + C[iir#c])) ==> (M[iir#c][idx$ - 0] == (M[iir#b][idx$ - 0] + M[iir#f][idx$ - 0]))
+  );
   assume R[iir#f] == (R[iir#c] + C[iir#c]);
+  assume (forall idx$: int :: 
+    (0 <= idx$) && (idx$ < (R[iir#c] + C[iir#c])) ==> (M[iir#c][idx$ - 0] == (M[iir#b][idx$ - 0] + M[iir#f][idx$ - 0]))
+  );
   assume R[iir#b] == (R[iir#c] + C[iir#c]);
+  assume (forall idx$: int :: 
+    (0 <= idx$) && (idx$ < (R[iir#g] + C[iir#g])) ==> (M[iir#g][idx$ - 0] == AT#RShift(M[iir#c][idx$ - 0], 8))
+  );
   assume R[iir#c] == (R[iir#g] + C[iir#g]);
+  assume (forall idx$: int :: 
+    (0 <= idx$) && (idx$ < (R[iir#d] + C[iir#d])) ==> (M[iir#d][idx$ - 0] == AT#RShift(M[iir#c][idx$ - 0], 8))
+  );
   assume R[iir#c] == (R[iir#d] + C[iir#d]);
+  assume (forall idx$: int :: 
+    (0 <= idx$) && (idx$ < (R[iir#e] + C[iir#e])) ==> (M[iir#e][idx$ - 0] == (171 * M[iir#d][idx$ - 0]))
+  );
   assume R[iir#d] == (R[iir#e] + C[iir#e]);
+  assume (forall idx$: int :: 
+    (0 <= idx$) && (idx$ < (R[iir#b] + C[iir#b])) ==> (M[iir#b][idx$ - 0] == (85 * M[iir#a][idx$ - 0]))
+  );
   assume R[iir#a] == (R[iir#b] + C[iir#b]);
+  assume (forall idx$: int :: 
+    (0 <= idx$) && (idx$ < ((R[iir#f] + C[iir#f]) - 1)) ==> (M[iir#f][(idx$ + 1) - 0] == M[iir#e][idx$ - 0])
+  );
   assume R[iir#e] == ((R[iir#f] + C[iir#f]) - 1);
   assume R[iir#g] == 0;
   assume 0 <= C[iir#g];
@@ -389,24 +425,6 @@ procedure iir#anon$5#mulc#anon$3#8()
   assume 0 <= C[iir#a];
   assume 0 <= R[iir#a];
   assume (171 * M[iir#g][-1]) == M[iir#f][0];
-  assume (forall i: int :: 
-    (0 <= i) && (i < (R[iir#b] + C[iir#b])) ==> (M[iir#b][i] == (85 * M[iir#a][i]))
-  );
-  assume (forall i: int :: 
-    (0 <= i) && (i < (R[iir#c] + C[iir#c])) ==> (M[iir#c][i] == (M[iir#b][i] + M[iir#f][i]))
-  );
-  assume (forall i: int :: 
-    (0 <= i) && (i < (R[iir#d] + C[iir#d])) ==> (M[iir#d][i] == AT#RShift(M[iir#c][i], 8))
-  );
-  assume (forall i: int :: 
-    (0 <= i) && (i < (R[iir#g] + C[iir#g])) ==> (M[iir#g][i] == AT#RShift(M[iir#c][i], 8))
-  );
-  assume (forall i: int :: 
-    (0 <= i) && (i < (R[iir#e] + C[iir#e])) ==> (M[iir#e][i] == (171 * M[iir#d][i]))
-  );
-  assume (forall i: int :: 
-    (1 <= i) && (i < (R[iir#f] + C[iir#f])) ==> (M[iir#f][i] == M[iir#e][i - 1])
-  );
   assume true;
   assume 1 <= C[iir#d];
   in#i := M[iir#d][R[iir#d]];
@@ -414,48 +432,51 @@ procedure iir#anon$5#mulc#anon$3#8()
   C[iir#d] := C[iir#d] - 1;
   M[iir#e][R[iir#e] + C[iir#e]] := ActorParam#c * in#i;
   C[iir#e] := C[iir#e] + 1;
-  assert {:msg "  Sub-actor action at 14.3 might not preserve the channel invariant (generated)"} R[iir#f] == (R[iir#c] + C[iir#c]);
-  assert {:msg "  Sub-actor action at 14.3 might not preserve the channel invariant (generated)"} R[iir#b] == (R[iir#c] + C[iir#c]);
-  assert {:msg "  Sub-actor action at 14.3 might not preserve the channel invariant (generated)"} R[iir#c] == (R[iir#g] + C[iir#g]);
-  assert {:msg "  Sub-actor action at 14.3 might not preserve the channel invariant (generated)"} R[iir#c] == (R[iir#d] + C[iir#d]);
-  assert {:msg "  Sub-actor action at 14.3 might not preserve the channel invariant (generated)"} R[iir#d] == (R[iir#e] + C[iir#e]);
-  assert {:msg "  Sub-actor action at 14.3 might not preserve the channel invariant (generated)"} R[iir#a] == (R[iir#b] + C[iir#b]);
-  assert {:msg "  Sub-actor action at 14.3 might not preserve the channel invariant (generated)"} R[iir#e] == ((R[iir#f] + C[iir#f]) - 1);
-  assert {:msg "  Sub-actor action at 14.3 might not preserve the channel invariant (generated)"} R[iir#g] == 0;
-  assert {:msg "  Sub-actor action at 14.3 might not preserve the channel invariant (generated)"} 0 <= C[iir#g];
-  assert {:msg "  Sub-actor action at 14.3 might not preserve the channel invariant (generated)"} 0 <= R[iir#g];
-  assert {:msg "  Sub-actor action at 14.3 might not preserve the channel invariant (generated)"} 0 <= C[iir#f];
-  assert {:msg "  Sub-actor action at 14.3 might not preserve the channel invariant (generated)"} 0 <= R[iir#f];
-  assert {:msg "  Sub-actor action at 14.3 might not preserve the channel invariant (generated)"} 0 <= C[iir#e];
-  assert {:msg "  Sub-actor action at 14.3 might not preserve the channel invariant (generated)"} 0 <= R[iir#e];
-  assert {:msg "  Sub-actor action at 14.3 might not preserve the channel invariant (generated)"} 0 <= C[iir#d];
-  assert {:msg "  Sub-actor action at 14.3 might not preserve the channel invariant (generated)"} 0 <= R[iir#d];
-  assert {:msg "  Sub-actor action at 14.3 might not preserve the channel invariant (generated)"} 0 <= C[iir#c];
-  assert {:msg "  Sub-actor action at 14.3 might not preserve the channel invariant (generated)"} 0 <= R[iir#c];
-  assert {:msg "  Sub-actor action at 14.3 might not preserve the channel invariant (generated)"} 0 <= C[iir#b];
-  assert {:msg "  Sub-actor action at 14.3 might not preserve the channel invariant (generated)"} 0 <= R[iir#b];
-  assert {:msg "  Sub-actor action at 14.3 might not preserve the channel invariant (generated)"} (R[iir#a] + C[iir#a]) == C#init[iir#a];
-  assert {:msg "  Sub-actor action at 14.3 might not preserve the channel invariant (generated)"} 0 <= C[iir#a];
-  assert {:msg "  Sub-actor action at 14.3 might not preserve the channel invariant (generated)"} 0 <= R[iir#a];
+  assert {:msg "  Sub-actor action at 14.3 might not preserve the channel invariant (generated #90)"} (forall idx$: int :: 
+    (0 <= idx$) && (idx$ < (R[iir#c] + C[iir#c])) ==> (M[iir#c][idx$ - 0] == (M[iir#b][idx$ - 0] + M[iir#f][idx$ - 0]))
+  );
+  assert {:msg "  Sub-actor action at 14.3 might not preserve the channel invariant (generated #91)"} R[iir#f] == (R[iir#c] + C[iir#c]);
+  assert {:msg "  Sub-actor action at 14.3 might not preserve the channel invariant (generated #92)"} (forall idx$: int :: 
+    (0 <= idx$) && (idx$ < (R[iir#c] + C[iir#c])) ==> (M[iir#c][idx$ - 0] == (M[iir#b][idx$ - 0] + M[iir#f][idx$ - 0]))
+  );
+  assert {:msg "  Sub-actor action at 14.3 might not preserve the channel invariant (generated #93)"} R[iir#b] == (R[iir#c] + C[iir#c]);
+  assert {:msg "  Sub-actor action at 14.3 might not preserve the channel invariant (generated #94)"} (forall idx$: int :: 
+    (0 <= idx$) && (idx$ < (R[iir#g] + C[iir#g])) ==> (M[iir#g][idx$ - 0] == AT#RShift(M[iir#c][idx$ - 0], 8))
+  );
+  assert {:msg "  Sub-actor action at 14.3 might not preserve the channel invariant (generated #95)"} R[iir#c] == (R[iir#g] + C[iir#g]);
+  assert {:msg "  Sub-actor action at 14.3 might not preserve the channel invariant (generated #96)"} (forall idx$: int :: 
+    (0 <= idx$) && (idx$ < (R[iir#d] + C[iir#d])) ==> (M[iir#d][idx$ - 0] == AT#RShift(M[iir#c][idx$ - 0], 8))
+  );
+  assert {:msg "  Sub-actor action at 14.3 might not preserve the channel invariant (generated #97)"} R[iir#c] == (R[iir#d] + C[iir#d]);
+  assert {:msg "  Sub-actor action at 14.3 might not preserve the channel invariant (generated #98)"} (forall idx$: int :: 
+    (0 <= idx$) && (idx$ < (R[iir#e] + C[iir#e])) ==> (M[iir#e][idx$ - 0] == (171 * M[iir#d][idx$ - 0]))
+  );
+  assert {:msg "  Sub-actor action at 14.3 might not preserve the channel invariant (generated #99)"} R[iir#d] == (R[iir#e] + C[iir#e]);
+  assert {:msg "  Sub-actor action at 14.3 might not preserve the channel invariant (generated #100)"} (forall idx$: int :: 
+    (0 <= idx$) && (idx$ < (R[iir#b] + C[iir#b])) ==> (M[iir#b][idx$ - 0] == (85 * M[iir#a][idx$ - 0]))
+  );
+  assert {:msg "  Sub-actor action at 14.3 might not preserve the channel invariant (generated #101)"} R[iir#a] == (R[iir#b] + C[iir#b]);
+  assert {:msg "  Sub-actor action at 14.3 might not preserve the channel invariant (generated #102)"} (forall idx$: int :: 
+    (0 <= idx$) && (idx$ < ((R[iir#f] + C[iir#f]) - 1)) ==> (M[iir#f][(idx$ + 1) - 0] == M[iir#e][idx$ - 0])
+  );
+  assert {:msg "  Sub-actor action at 14.3 might not preserve the channel invariant (generated #103)"} R[iir#e] == ((R[iir#f] + C[iir#f]) - 1);
+  assert {:msg "  Sub-actor action at 14.3 might not preserve the channel invariant (generated #104)"} R[iir#g] == 0;
+  assert {:msg "  Sub-actor action at 14.3 might not preserve the channel invariant (generated #105)"} 0 <= C[iir#g];
+  assert {:msg "  Sub-actor action at 14.3 might not preserve the channel invariant (generated #106)"} 0 <= R[iir#g];
+  assert {:msg "  Sub-actor action at 14.3 might not preserve the channel invariant (generated #107)"} 0 <= C[iir#f];
+  assert {:msg "  Sub-actor action at 14.3 might not preserve the channel invariant (generated #108)"} 0 <= R[iir#f];
+  assert {:msg "  Sub-actor action at 14.3 might not preserve the channel invariant (generated #109)"} 0 <= C[iir#e];
+  assert {:msg "  Sub-actor action at 14.3 might not preserve the channel invariant (generated #110)"} 0 <= R[iir#e];
+  assert {:msg "  Sub-actor action at 14.3 might not preserve the channel invariant (generated #111)"} 0 <= C[iir#d];
+  assert {:msg "  Sub-actor action at 14.3 might not preserve the channel invariant (generated #112)"} 0 <= R[iir#d];
+  assert {:msg "  Sub-actor action at 14.3 might not preserve the channel invariant (generated #113)"} 0 <= C[iir#c];
+  assert {:msg "  Sub-actor action at 14.3 might not preserve the channel invariant (generated #114)"} 0 <= R[iir#c];
+  assert {:msg "  Sub-actor action at 14.3 might not preserve the channel invariant (generated #115)"} 0 <= C[iir#b];
+  assert {:msg "  Sub-actor action at 14.3 might not preserve the channel invariant (generated #116)"} 0 <= R[iir#b];
+  assert {:msg "  Sub-actor action at 14.3 might not preserve the channel invariant (generated #117)"} (R[iir#a] + C[iir#a]) == C#init[iir#a];
+  assert {:msg "  Sub-actor action at 14.3 might not preserve the channel invariant (generated #118)"} 0 <= C[iir#a];
+  assert {:msg "  Sub-actor action at 14.3 might not preserve the channel invariant (generated #119)"} 0 <= R[iir#a];
   assert {:msg "  28.3: Sub-actor action at 14.3 might not preserve the channel invariant"} (171 * M[iir#g][-1]) == M[iir#f][0];
-  assert {:msg "  29.3: Sub-actor action at 14.3 might not preserve the channel invariant"} (forall i: int :: 
-    (0 <= i) && (i < (R[iir#b] + C[iir#b])) ==> (M[iir#b][i] == (85 * M[iir#a][i]))
-  );
-  assert {:msg "  30.3: Sub-actor action at 14.3 might not preserve the channel invariant"} (forall i: int :: 
-    (0 <= i) && (i < (R[iir#c] + C[iir#c])) ==> (M[iir#c][i] == (M[iir#b][i] + M[iir#f][i]))
-  );
-  assert {:msg "  31.3: Sub-actor action at 14.3 might not preserve the channel invariant"} (forall i: int :: 
-    (0 <= i) && (i < (R[iir#d] + C[iir#d])) ==> (M[iir#d][i] == AT#RShift(M[iir#c][i], 8))
-  );
-  assert {:msg "  32.3: Sub-actor action at 14.3 might not preserve the channel invariant"} (forall i: int :: 
-    (0 <= i) && (i < (R[iir#g] + C[iir#g])) ==> (M[iir#g][i] == AT#RShift(M[iir#c][i], 8))
-  );
-  assert {:msg "  33.3: Sub-actor action at 14.3 might not preserve the channel invariant"} (forall i: int :: 
-    (0 <= i) && (i < (R[iir#e] + C[iir#e])) ==> (M[iir#e][i] == (171 * M[iir#d][i]))
-  );
-  assert {:msg "  34.3: Sub-actor action at 14.3 might not preserve the channel invariant"} (forall i: int :: 
-    (1 <= i) && (i < (R[iir#f] + C[iir#f])) ==> (M[iir#f][i] == M[iir#e][i - 1])
-  );
 }
 procedure iir#anon$5#rshift#anon$4#9()
   modifies C, R, M, St;
@@ -470,12 +491,33 @@ procedure iir#anon$5#rshift#anon$4#9()
   assume C#init[iir#d] == 0;
   assume C#init[iir#e] == 0;
   assume C#init[iir#g] == 0;
+  assume (forall idx$: int :: 
+    (0 <= idx$) && (idx$ < (R[iir#c] + C[iir#c])) ==> (M[iir#c][idx$ - 0] == (M[iir#b][idx$ - 0] + M[iir#f][idx$ - 0]))
+  );
   assume R[iir#f] == (R[iir#c] + C[iir#c]);
+  assume (forall idx$: int :: 
+    (0 <= idx$) && (idx$ < (R[iir#c] + C[iir#c])) ==> (M[iir#c][idx$ - 0] == (M[iir#b][idx$ - 0] + M[iir#f][idx$ - 0]))
+  );
   assume R[iir#b] == (R[iir#c] + C[iir#c]);
+  assume (forall idx$: int :: 
+    (0 <= idx$) && (idx$ < (R[iir#g] + C[iir#g])) ==> (M[iir#g][idx$ - 0] == AT#RShift(M[iir#c][idx$ - 0], 8))
+  );
   assume R[iir#c] == (R[iir#g] + C[iir#g]);
+  assume (forall idx$: int :: 
+    (0 <= idx$) && (idx$ < (R[iir#d] + C[iir#d])) ==> (M[iir#d][idx$ - 0] == AT#RShift(M[iir#c][idx$ - 0], 8))
+  );
   assume R[iir#c] == (R[iir#d] + C[iir#d]);
+  assume (forall idx$: int :: 
+    (0 <= idx$) && (idx$ < (R[iir#e] + C[iir#e])) ==> (M[iir#e][idx$ - 0] == (171 * M[iir#d][idx$ - 0]))
+  );
   assume R[iir#d] == (R[iir#e] + C[iir#e]);
+  assume (forall idx$: int :: 
+    (0 <= idx$) && (idx$ < (R[iir#b] + C[iir#b])) ==> (M[iir#b][idx$ - 0] == (85 * M[iir#a][idx$ - 0]))
+  );
   assume R[iir#a] == (R[iir#b] + C[iir#b]);
+  assume (forall idx$: int :: 
+    (0 <= idx$) && (idx$ < ((R[iir#f] + C[iir#f]) - 1)) ==> (M[iir#f][(idx$ + 1) - 0] == M[iir#e][idx$ - 0])
+  );
   assume R[iir#e] == ((R[iir#f] + C[iir#f]) - 1);
   assume R[iir#g] == 0;
   assume 0 <= C[iir#g];
@@ -494,24 +536,6 @@ procedure iir#anon$5#rshift#anon$4#9()
   assume 0 <= C[iir#a];
   assume 0 <= R[iir#a];
   assume (171 * M[iir#g][-1]) == M[iir#f][0];
-  assume (forall i: int :: 
-    (0 <= i) && (i < (R[iir#b] + C[iir#b])) ==> (M[iir#b][i] == (85 * M[iir#a][i]))
-  );
-  assume (forall i: int :: 
-    (0 <= i) && (i < (R[iir#c] + C[iir#c])) ==> (M[iir#c][i] == (M[iir#b][i] + M[iir#f][i]))
-  );
-  assume (forall i: int :: 
-    (0 <= i) && (i < (R[iir#d] + C[iir#d])) ==> (M[iir#d][i] == AT#RShift(M[iir#c][i], 8))
-  );
-  assume (forall i: int :: 
-    (0 <= i) && (i < (R[iir#g] + C[iir#g])) ==> (M[iir#g][i] == AT#RShift(M[iir#c][i], 8))
-  );
-  assume (forall i: int :: 
-    (0 <= i) && (i < (R[iir#e] + C[iir#e])) ==> (M[iir#e][i] == (171 * M[iir#d][i]))
-  );
-  assume (forall i: int :: 
-    (1 <= i) && (i < (R[iir#f] + C[iir#f])) ==> (M[iir#f][i] == M[iir#e][i - 1])
-  );
   assume true;
   assume 1 <= C[iir#c];
   in#i := M[iir#c][R[iir#c]];
@@ -521,48 +545,51 @@ procedure iir#anon$5#rshift#anon$4#9()
   C[iir#d] := C[iir#d] + 1;
   M[iir#g][R[iir#g] + C[iir#g]] := AT#RShift(in#i, ActorParam#s);
   C[iir#g] := C[iir#g] + 1;
-  assert {:msg "  Sub-actor action at 19.3 might not preserve the channel invariant (generated)"} R[iir#f] == (R[iir#c] + C[iir#c]);
-  assert {:msg "  Sub-actor action at 19.3 might not preserve the channel invariant (generated)"} R[iir#b] == (R[iir#c] + C[iir#c]);
-  assert {:msg "  Sub-actor action at 19.3 might not preserve the channel invariant (generated)"} R[iir#c] == (R[iir#g] + C[iir#g]);
-  assert {:msg "  Sub-actor action at 19.3 might not preserve the channel invariant (generated)"} R[iir#c] == (R[iir#d] + C[iir#d]);
-  assert {:msg "  Sub-actor action at 19.3 might not preserve the channel invariant (generated)"} R[iir#d] == (R[iir#e] + C[iir#e]);
-  assert {:msg "  Sub-actor action at 19.3 might not preserve the channel invariant (generated)"} R[iir#a] == (R[iir#b] + C[iir#b]);
-  assert {:msg "  Sub-actor action at 19.3 might not preserve the channel invariant (generated)"} R[iir#e] == ((R[iir#f] + C[iir#f]) - 1);
-  assert {:msg "  Sub-actor action at 19.3 might not preserve the channel invariant (generated)"} R[iir#g] == 0;
-  assert {:msg "  Sub-actor action at 19.3 might not preserve the channel invariant (generated)"} 0 <= C[iir#g];
-  assert {:msg "  Sub-actor action at 19.3 might not preserve the channel invariant (generated)"} 0 <= R[iir#g];
-  assert {:msg "  Sub-actor action at 19.3 might not preserve the channel invariant (generated)"} 0 <= C[iir#f];
-  assert {:msg "  Sub-actor action at 19.3 might not preserve the channel invariant (generated)"} 0 <= R[iir#f];
-  assert {:msg "  Sub-actor action at 19.3 might not preserve the channel invariant (generated)"} 0 <= C[iir#e];
-  assert {:msg "  Sub-actor action at 19.3 might not preserve the channel invariant (generated)"} 0 <= R[iir#e];
-  assert {:msg "  Sub-actor action at 19.3 might not preserve the channel invariant (generated)"} 0 <= C[iir#d];
-  assert {:msg "  Sub-actor action at 19.3 might not preserve the channel invariant (generated)"} 0 <= R[iir#d];
-  assert {:msg "  Sub-actor action at 19.3 might not preserve the channel invariant (generated)"} 0 <= C[iir#c];
-  assert {:msg "  Sub-actor action at 19.3 might not preserve the channel invariant (generated)"} 0 <= R[iir#c];
-  assert {:msg "  Sub-actor action at 19.3 might not preserve the channel invariant (generated)"} 0 <= C[iir#b];
-  assert {:msg "  Sub-actor action at 19.3 might not preserve the channel invariant (generated)"} 0 <= R[iir#b];
-  assert {:msg "  Sub-actor action at 19.3 might not preserve the channel invariant (generated)"} (R[iir#a] + C[iir#a]) == C#init[iir#a];
-  assert {:msg "  Sub-actor action at 19.3 might not preserve the channel invariant (generated)"} 0 <= C[iir#a];
-  assert {:msg "  Sub-actor action at 19.3 might not preserve the channel invariant (generated)"} 0 <= R[iir#a];
+  assert {:msg "  Sub-actor action at 19.3 might not preserve the channel invariant (generated #120)"} (forall idx$: int :: 
+    (0 <= idx$) && (idx$ < (R[iir#c] + C[iir#c])) ==> (M[iir#c][idx$ - 0] == (M[iir#b][idx$ - 0] + M[iir#f][idx$ - 0]))
+  );
+  assert {:msg "  Sub-actor action at 19.3 might not preserve the channel invariant (generated #121)"} R[iir#f] == (R[iir#c] + C[iir#c]);
+  assert {:msg "  Sub-actor action at 19.3 might not preserve the channel invariant (generated #122)"} (forall idx$: int :: 
+    (0 <= idx$) && (idx$ < (R[iir#c] + C[iir#c])) ==> (M[iir#c][idx$ - 0] == (M[iir#b][idx$ - 0] + M[iir#f][idx$ - 0]))
+  );
+  assert {:msg "  Sub-actor action at 19.3 might not preserve the channel invariant (generated #123)"} R[iir#b] == (R[iir#c] + C[iir#c]);
+  assert {:msg "  Sub-actor action at 19.3 might not preserve the channel invariant (generated #124)"} (forall idx$: int :: 
+    (0 <= idx$) && (idx$ < (R[iir#g] + C[iir#g])) ==> (M[iir#g][idx$ - 0] == AT#RShift(M[iir#c][idx$ - 0], 8))
+  );
+  assert {:msg "  Sub-actor action at 19.3 might not preserve the channel invariant (generated #125)"} R[iir#c] == (R[iir#g] + C[iir#g]);
+  assert {:msg "  Sub-actor action at 19.3 might not preserve the channel invariant (generated #126)"} (forall idx$: int :: 
+    (0 <= idx$) && (idx$ < (R[iir#d] + C[iir#d])) ==> (M[iir#d][idx$ - 0] == AT#RShift(M[iir#c][idx$ - 0], 8))
+  );
+  assert {:msg "  Sub-actor action at 19.3 might not preserve the channel invariant (generated #127)"} R[iir#c] == (R[iir#d] + C[iir#d]);
+  assert {:msg "  Sub-actor action at 19.3 might not preserve the channel invariant (generated #128)"} (forall idx$: int :: 
+    (0 <= idx$) && (idx$ < (R[iir#e] + C[iir#e])) ==> (M[iir#e][idx$ - 0] == (171 * M[iir#d][idx$ - 0]))
+  );
+  assert {:msg "  Sub-actor action at 19.3 might not preserve the channel invariant (generated #129)"} R[iir#d] == (R[iir#e] + C[iir#e]);
+  assert {:msg "  Sub-actor action at 19.3 might not preserve the channel invariant (generated #130)"} (forall idx$: int :: 
+    (0 <= idx$) && (idx$ < (R[iir#b] + C[iir#b])) ==> (M[iir#b][idx$ - 0] == (85 * M[iir#a][idx$ - 0]))
+  );
+  assert {:msg "  Sub-actor action at 19.3 might not preserve the channel invariant (generated #131)"} R[iir#a] == (R[iir#b] + C[iir#b]);
+  assert {:msg "  Sub-actor action at 19.3 might not preserve the channel invariant (generated #132)"} (forall idx$: int :: 
+    (0 <= idx$) && (idx$ < ((R[iir#f] + C[iir#f]) - 1)) ==> (M[iir#f][(idx$ + 1) - 0] == M[iir#e][idx$ - 0])
+  );
+  assert {:msg "  Sub-actor action at 19.3 might not preserve the channel invariant (generated #133)"} R[iir#e] == ((R[iir#f] + C[iir#f]) - 1);
+  assert {:msg "  Sub-actor action at 19.3 might not preserve the channel invariant (generated #134)"} R[iir#g] == 0;
+  assert {:msg "  Sub-actor action at 19.3 might not preserve the channel invariant (generated #135)"} 0 <= C[iir#g];
+  assert {:msg "  Sub-actor action at 19.3 might not preserve the channel invariant (generated #136)"} 0 <= R[iir#g];
+  assert {:msg "  Sub-actor action at 19.3 might not preserve the channel invariant (generated #137)"} 0 <= C[iir#f];
+  assert {:msg "  Sub-actor action at 19.3 might not preserve the channel invariant (generated #138)"} 0 <= R[iir#f];
+  assert {:msg "  Sub-actor action at 19.3 might not preserve the channel invariant (generated #139)"} 0 <= C[iir#e];
+  assert {:msg "  Sub-actor action at 19.3 might not preserve the channel invariant (generated #140)"} 0 <= R[iir#e];
+  assert {:msg "  Sub-actor action at 19.3 might not preserve the channel invariant (generated #141)"} 0 <= C[iir#d];
+  assert {:msg "  Sub-actor action at 19.3 might not preserve the channel invariant (generated #142)"} 0 <= R[iir#d];
+  assert {:msg "  Sub-actor action at 19.3 might not preserve the channel invariant (generated #143)"} 0 <= C[iir#c];
+  assert {:msg "  Sub-actor action at 19.3 might not preserve the channel invariant (generated #144)"} 0 <= R[iir#c];
+  assert {:msg "  Sub-actor action at 19.3 might not preserve the channel invariant (generated #145)"} 0 <= C[iir#b];
+  assert {:msg "  Sub-actor action at 19.3 might not preserve the channel invariant (generated #146)"} 0 <= R[iir#b];
+  assert {:msg "  Sub-actor action at 19.3 might not preserve the channel invariant (generated #147)"} (R[iir#a] + C[iir#a]) == C#init[iir#a];
+  assert {:msg "  Sub-actor action at 19.3 might not preserve the channel invariant (generated #148)"} 0 <= C[iir#a];
+  assert {:msg "  Sub-actor action at 19.3 might not preserve the channel invariant (generated #149)"} 0 <= R[iir#a];
   assert {:msg "  28.3: Sub-actor action at 19.3 might not preserve the channel invariant"} (171 * M[iir#g][-1]) == M[iir#f][0];
-  assert {:msg "  29.3: Sub-actor action at 19.3 might not preserve the channel invariant"} (forall i: int :: 
-    (0 <= i) && (i < (R[iir#b] + C[iir#b])) ==> (M[iir#b][i] == (85 * M[iir#a][i]))
-  );
-  assert {:msg "  30.3: Sub-actor action at 19.3 might not preserve the channel invariant"} (forall i: int :: 
-    (0 <= i) && (i < (R[iir#c] + C[iir#c])) ==> (M[iir#c][i] == (M[iir#b][i] + M[iir#f][i]))
-  );
-  assert {:msg "  31.3: Sub-actor action at 19.3 might not preserve the channel invariant"} (forall i: int :: 
-    (0 <= i) && (i < (R[iir#d] + C[iir#d])) ==> (M[iir#d][i] == AT#RShift(M[iir#c][i], 8))
-  );
-  assert {:msg "  32.3: Sub-actor action at 19.3 might not preserve the channel invariant"} (forall i: int :: 
-    (0 <= i) && (i < (R[iir#g] + C[iir#g])) ==> (M[iir#g][i] == AT#RShift(M[iir#c][i], 8))
-  );
-  assert {:msg "  33.3: Sub-actor action at 19.3 might not preserve the channel invariant"} (forall i: int :: 
-    (0 <= i) && (i < (R[iir#e] + C[iir#e])) ==> (M[iir#e][i] == (171 * M[iir#d][i]))
-  );
-  assert {:msg "  34.3: Sub-actor action at 19.3 might not preserve the channel invariant"} (forall i: int :: 
-    (1 <= i) && (i < (R[iir#f] + C[iir#f])) ==> (M[iir#f][i] == M[iir#e][i - 1])
-  );
 }
 procedure iir#anon$5#add#anon$0#10()
   modifies C, R, M, St;
@@ -576,12 +603,33 @@ procedure iir#anon$5#add#anon$0#10()
   assume C#init[iir#d] == 0;
   assume C#init[iir#e] == 0;
   assume C#init[iir#g] == 0;
+  assume (forall idx$: int :: 
+    (0 <= idx$) && (idx$ < (R[iir#c] + C[iir#c])) ==> (M[iir#c][idx$ - 0] == (M[iir#b][idx$ - 0] + M[iir#f][idx$ - 0]))
+  );
   assume R[iir#f] == (R[iir#c] + C[iir#c]);
+  assume (forall idx$: int :: 
+    (0 <= idx$) && (idx$ < (R[iir#c] + C[iir#c])) ==> (M[iir#c][idx$ - 0] == (M[iir#b][idx$ - 0] + M[iir#f][idx$ - 0]))
+  );
   assume R[iir#b] == (R[iir#c] + C[iir#c]);
+  assume (forall idx$: int :: 
+    (0 <= idx$) && (idx$ < (R[iir#g] + C[iir#g])) ==> (M[iir#g][idx$ - 0] == AT#RShift(M[iir#c][idx$ - 0], 8))
+  );
   assume R[iir#c] == (R[iir#g] + C[iir#g]);
+  assume (forall idx$: int :: 
+    (0 <= idx$) && (idx$ < (R[iir#d] + C[iir#d])) ==> (M[iir#d][idx$ - 0] == AT#RShift(M[iir#c][idx$ - 0], 8))
+  );
   assume R[iir#c] == (R[iir#d] + C[iir#d]);
+  assume (forall idx$: int :: 
+    (0 <= idx$) && (idx$ < (R[iir#e] + C[iir#e])) ==> (M[iir#e][idx$ - 0] == (171 * M[iir#d][idx$ - 0]))
+  );
   assume R[iir#d] == (R[iir#e] + C[iir#e]);
+  assume (forall idx$: int :: 
+    (0 <= idx$) && (idx$ < (R[iir#b] + C[iir#b])) ==> (M[iir#b][idx$ - 0] == (85 * M[iir#a][idx$ - 0]))
+  );
   assume R[iir#a] == (R[iir#b] + C[iir#b]);
+  assume (forall idx$: int :: 
+    (0 <= idx$) && (idx$ < ((R[iir#f] + C[iir#f]) - 1)) ==> (M[iir#f][(idx$ + 1) - 0] == M[iir#e][idx$ - 0])
+  );
   assume R[iir#e] == ((R[iir#f] + C[iir#f]) - 1);
   assume R[iir#g] == 0;
   assume 0 <= C[iir#g];
@@ -600,24 +648,6 @@ procedure iir#anon$5#add#anon$0#10()
   assume 0 <= C[iir#a];
   assume 0 <= R[iir#a];
   assume (171 * M[iir#g][-1]) == M[iir#f][0];
-  assume (forall i: int :: 
-    (0 <= i) && (i < (R[iir#b] + C[iir#b])) ==> (M[iir#b][i] == (85 * M[iir#a][i]))
-  );
-  assume (forall i: int :: 
-    (0 <= i) && (i < (R[iir#c] + C[iir#c])) ==> (M[iir#c][i] == (M[iir#b][i] + M[iir#f][i]))
-  );
-  assume (forall i: int :: 
-    (0 <= i) && (i < (R[iir#d] + C[iir#d])) ==> (M[iir#d][i] == AT#RShift(M[iir#c][i], 8))
-  );
-  assume (forall i: int :: 
-    (0 <= i) && (i < (R[iir#g] + C[iir#g])) ==> (M[iir#g][i] == AT#RShift(M[iir#c][i], 8))
-  );
-  assume (forall i: int :: 
-    (0 <= i) && (i < (R[iir#e] + C[iir#e])) ==> (M[iir#e][i] == (171 * M[iir#d][i]))
-  );
-  assume (forall i: int :: 
-    (1 <= i) && (i < (R[iir#f] + C[iir#f])) ==> (M[iir#f][i] == M[iir#e][i - 1])
-  );
   assume true;
   assume (1 <= C[iir#b]) && (1 <= C[iir#f]);
   in1#i := M[iir#b][R[iir#b]];
@@ -628,48 +658,51 @@ procedure iir#anon$5#add#anon$0#10()
   C[iir#f] := C[iir#f] - 1;
   M[iir#c][R[iir#c] + C[iir#c]] := in1#i + in2#j;
   C[iir#c] := C[iir#c] + 1;
-  assert {:msg "  Sub-actor action at 3.3 might not preserve the channel invariant (generated)"} R[iir#f] == (R[iir#c] + C[iir#c]);
-  assert {:msg "  Sub-actor action at 3.3 might not preserve the channel invariant (generated)"} R[iir#b] == (R[iir#c] + C[iir#c]);
-  assert {:msg "  Sub-actor action at 3.3 might not preserve the channel invariant (generated)"} R[iir#c] == (R[iir#g] + C[iir#g]);
-  assert {:msg "  Sub-actor action at 3.3 might not preserve the channel invariant (generated)"} R[iir#c] == (R[iir#d] + C[iir#d]);
-  assert {:msg "  Sub-actor action at 3.3 might not preserve the channel invariant (generated)"} R[iir#d] == (R[iir#e] + C[iir#e]);
-  assert {:msg "  Sub-actor action at 3.3 might not preserve the channel invariant (generated)"} R[iir#a] == (R[iir#b] + C[iir#b]);
-  assert {:msg "  Sub-actor action at 3.3 might not preserve the channel invariant (generated)"} R[iir#e] == ((R[iir#f] + C[iir#f]) - 1);
-  assert {:msg "  Sub-actor action at 3.3 might not preserve the channel invariant (generated)"} R[iir#g] == 0;
-  assert {:msg "  Sub-actor action at 3.3 might not preserve the channel invariant (generated)"} 0 <= C[iir#g];
-  assert {:msg "  Sub-actor action at 3.3 might not preserve the channel invariant (generated)"} 0 <= R[iir#g];
-  assert {:msg "  Sub-actor action at 3.3 might not preserve the channel invariant (generated)"} 0 <= C[iir#f];
-  assert {:msg "  Sub-actor action at 3.3 might not preserve the channel invariant (generated)"} 0 <= R[iir#f];
-  assert {:msg "  Sub-actor action at 3.3 might not preserve the channel invariant (generated)"} 0 <= C[iir#e];
-  assert {:msg "  Sub-actor action at 3.3 might not preserve the channel invariant (generated)"} 0 <= R[iir#e];
-  assert {:msg "  Sub-actor action at 3.3 might not preserve the channel invariant (generated)"} 0 <= C[iir#d];
-  assert {:msg "  Sub-actor action at 3.3 might not preserve the channel invariant (generated)"} 0 <= R[iir#d];
-  assert {:msg "  Sub-actor action at 3.3 might not preserve the channel invariant (generated)"} 0 <= C[iir#c];
-  assert {:msg "  Sub-actor action at 3.3 might not preserve the channel invariant (generated)"} 0 <= R[iir#c];
-  assert {:msg "  Sub-actor action at 3.3 might not preserve the channel invariant (generated)"} 0 <= C[iir#b];
-  assert {:msg "  Sub-actor action at 3.3 might not preserve the channel invariant (generated)"} 0 <= R[iir#b];
-  assert {:msg "  Sub-actor action at 3.3 might not preserve the channel invariant (generated)"} (R[iir#a] + C[iir#a]) == C#init[iir#a];
-  assert {:msg "  Sub-actor action at 3.3 might not preserve the channel invariant (generated)"} 0 <= C[iir#a];
-  assert {:msg "  Sub-actor action at 3.3 might not preserve the channel invariant (generated)"} 0 <= R[iir#a];
+  assert {:msg "  Sub-actor action at 3.3 might not preserve the channel invariant (generated #150)"} (forall idx$: int :: 
+    (0 <= idx$) && (idx$ < (R[iir#c] + C[iir#c])) ==> (M[iir#c][idx$ - 0] == (M[iir#b][idx$ - 0] + M[iir#f][idx$ - 0]))
+  );
+  assert {:msg "  Sub-actor action at 3.3 might not preserve the channel invariant (generated #151)"} R[iir#f] == (R[iir#c] + C[iir#c]);
+  assert {:msg "  Sub-actor action at 3.3 might not preserve the channel invariant (generated #152)"} (forall idx$: int :: 
+    (0 <= idx$) && (idx$ < (R[iir#c] + C[iir#c])) ==> (M[iir#c][idx$ - 0] == (M[iir#b][idx$ - 0] + M[iir#f][idx$ - 0]))
+  );
+  assert {:msg "  Sub-actor action at 3.3 might not preserve the channel invariant (generated #153)"} R[iir#b] == (R[iir#c] + C[iir#c]);
+  assert {:msg "  Sub-actor action at 3.3 might not preserve the channel invariant (generated #154)"} (forall idx$: int :: 
+    (0 <= idx$) && (idx$ < (R[iir#g] + C[iir#g])) ==> (M[iir#g][idx$ - 0] == AT#RShift(M[iir#c][idx$ - 0], 8))
+  );
+  assert {:msg "  Sub-actor action at 3.3 might not preserve the channel invariant (generated #155)"} R[iir#c] == (R[iir#g] + C[iir#g]);
+  assert {:msg "  Sub-actor action at 3.3 might not preserve the channel invariant (generated #156)"} (forall idx$: int :: 
+    (0 <= idx$) && (idx$ < (R[iir#d] + C[iir#d])) ==> (M[iir#d][idx$ - 0] == AT#RShift(M[iir#c][idx$ - 0], 8))
+  );
+  assert {:msg "  Sub-actor action at 3.3 might not preserve the channel invariant (generated #157)"} R[iir#c] == (R[iir#d] + C[iir#d]);
+  assert {:msg "  Sub-actor action at 3.3 might not preserve the channel invariant (generated #158)"} (forall idx$: int :: 
+    (0 <= idx$) && (idx$ < (R[iir#e] + C[iir#e])) ==> (M[iir#e][idx$ - 0] == (171 * M[iir#d][idx$ - 0]))
+  );
+  assert {:msg "  Sub-actor action at 3.3 might not preserve the channel invariant (generated #159)"} R[iir#d] == (R[iir#e] + C[iir#e]);
+  assert {:msg "  Sub-actor action at 3.3 might not preserve the channel invariant (generated #160)"} (forall idx$: int :: 
+    (0 <= idx$) && (idx$ < (R[iir#b] + C[iir#b])) ==> (M[iir#b][idx$ - 0] == (85 * M[iir#a][idx$ - 0]))
+  );
+  assert {:msg "  Sub-actor action at 3.3 might not preserve the channel invariant (generated #161)"} R[iir#a] == (R[iir#b] + C[iir#b]);
+  assert {:msg "  Sub-actor action at 3.3 might not preserve the channel invariant (generated #162)"} (forall idx$: int :: 
+    (0 <= idx$) && (idx$ < ((R[iir#f] + C[iir#f]) - 1)) ==> (M[iir#f][(idx$ + 1) - 0] == M[iir#e][idx$ - 0])
+  );
+  assert {:msg "  Sub-actor action at 3.3 might not preserve the channel invariant (generated #163)"} R[iir#e] == ((R[iir#f] + C[iir#f]) - 1);
+  assert {:msg "  Sub-actor action at 3.3 might not preserve the channel invariant (generated #164)"} R[iir#g] == 0;
+  assert {:msg "  Sub-actor action at 3.3 might not preserve the channel invariant (generated #165)"} 0 <= C[iir#g];
+  assert {:msg "  Sub-actor action at 3.3 might not preserve the channel invariant (generated #166)"} 0 <= R[iir#g];
+  assert {:msg "  Sub-actor action at 3.3 might not preserve the channel invariant (generated #167)"} 0 <= C[iir#f];
+  assert {:msg "  Sub-actor action at 3.3 might not preserve the channel invariant (generated #168)"} 0 <= R[iir#f];
+  assert {:msg "  Sub-actor action at 3.3 might not preserve the channel invariant (generated #169)"} 0 <= C[iir#e];
+  assert {:msg "  Sub-actor action at 3.3 might not preserve the channel invariant (generated #170)"} 0 <= R[iir#e];
+  assert {:msg "  Sub-actor action at 3.3 might not preserve the channel invariant (generated #171)"} 0 <= C[iir#d];
+  assert {:msg "  Sub-actor action at 3.3 might not preserve the channel invariant (generated #172)"} 0 <= R[iir#d];
+  assert {:msg "  Sub-actor action at 3.3 might not preserve the channel invariant (generated #173)"} 0 <= C[iir#c];
+  assert {:msg "  Sub-actor action at 3.3 might not preserve the channel invariant (generated #174)"} 0 <= R[iir#c];
+  assert {:msg "  Sub-actor action at 3.3 might not preserve the channel invariant (generated #175)"} 0 <= C[iir#b];
+  assert {:msg "  Sub-actor action at 3.3 might not preserve the channel invariant (generated #176)"} 0 <= R[iir#b];
+  assert {:msg "  Sub-actor action at 3.3 might not preserve the channel invariant (generated #177)"} (R[iir#a] + C[iir#a]) == C#init[iir#a];
+  assert {:msg "  Sub-actor action at 3.3 might not preserve the channel invariant (generated #178)"} 0 <= C[iir#a];
+  assert {:msg "  Sub-actor action at 3.3 might not preserve the channel invariant (generated #179)"} 0 <= R[iir#a];
   assert {:msg "  28.3: Sub-actor action at 3.3 might not preserve the channel invariant"} (171 * M[iir#g][-1]) == M[iir#f][0];
-  assert {:msg "  29.3: Sub-actor action at 3.3 might not preserve the channel invariant"} (forall i: int :: 
-    (0 <= i) && (i < (R[iir#b] + C[iir#b])) ==> (M[iir#b][i] == (85 * M[iir#a][i]))
-  );
-  assert {:msg "  30.3: Sub-actor action at 3.3 might not preserve the channel invariant"} (forall i: int :: 
-    (0 <= i) && (i < (R[iir#c] + C[iir#c])) ==> (M[iir#c][i] == (M[iir#b][i] + M[iir#f][i]))
-  );
-  assert {:msg "  31.3: Sub-actor action at 3.3 might not preserve the channel invariant"} (forall i: int :: 
-    (0 <= i) && (i < (R[iir#d] + C[iir#d])) ==> (M[iir#d][i] == AT#RShift(M[iir#c][i], 8))
-  );
-  assert {:msg "  32.3: Sub-actor action at 3.3 might not preserve the channel invariant"} (forall i: int :: 
-    (0 <= i) && (i < (R[iir#g] + C[iir#g])) ==> (M[iir#g][i] == AT#RShift(M[iir#c][i], 8))
-  );
-  assert {:msg "  33.3: Sub-actor action at 3.3 might not preserve the channel invariant"} (forall i: int :: 
-    (0 <= i) && (i < (R[iir#e] + C[iir#e])) ==> (M[iir#e][i] == (171 * M[iir#d][i]))
-  );
-  assert {:msg "  34.3: Sub-actor action at 3.3 might not preserve the channel invariant"} (forall i: int :: 
-    (1 <= i) && (i < (R[iir#f] + C[iir#f])) ==> (M[iir#f][i] == M[iir#e][i - 1])
-  );
 }
 procedure iir#anon$5#exit#11()
   modifies C, R, M, St;
@@ -680,12 +713,33 @@ procedure iir#anon$5#exit#11()
   assume C#init[iir#d] == 0;
   assume C#init[iir#e] == 0;
   assume C#init[iir#g] == 0;
+  assume (forall idx$: int :: 
+    (0 <= idx$) && (idx$ < (R[iir#c] + C[iir#c])) ==> (M[iir#c][idx$ - 0] == (M[iir#b][idx$ - 0] + M[iir#f][idx$ - 0]))
+  );
   assume R[iir#f] == (R[iir#c] + C[iir#c]);
+  assume (forall idx$: int :: 
+    (0 <= idx$) && (idx$ < (R[iir#c] + C[iir#c])) ==> (M[iir#c][idx$ - 0] == (M[iir#b][idx$ - 0] + M[iir#f][idx$ - 0]))
+  );
   assume R[iir#b] == (R[iir#c] + C[iir#c]);
+  assume (forall idx$: int :: 
+    (0 <= idx$) && (idx$ < (R[iir#g] + C[iir#g])) ==> (M[iir#g][idx$ - 0] == AT#RShift(M[iir#c][idx$ - 0], 8))
+  );
   assume R[iir#c] == (R[iir#g] + C[iir#g]);
+  assume (forall idx$: int :: 
+    (0 <= idx$) && (idx$ < (R[iir#d] + C[iir#d])) ==> (M[iir#d][idx$ - 0] == AT#RShift(M[iir#c][idx$ - 0], 8))
+  );
   assume R[iir#c] == (R[iir#d] + C[iir#d]);
+  assume (forall idx$: int :: 
+    (0 <= idx$) && (idx$ < (R[iir#e] + C[iir#e])) ==> (M[iir#e][idx$ - 0] == (171 * M[iir#d][idx$ - 0]))
+  );
   assume R[iir#d] == (R[iir#e] + C[iir#e]);
+  assume (forall idx$: int :: 
+    (0 <= idx$) && (idx$ < (R[iir#b] + C[iir#b])) ==> (M[iir#b][idx$ - 0] == (85 * M[iir#a][idx$ - 0]))
+  );
   assume R[iir#a] == (R[iir#b] + C[iir#b]);
+  assume (forall idx$: int :: 
+    (0 <= idx$) && (idx$ < ((R[iir#f] + C[iir#f]) - 1)) ==> (M[iir#f][(idx$ + 1) - 0] == M[iir#e][idx$ - 0])
+  );
   assume R[iir#e] == ((R[iir#f] + C[iir#f]) - 1);
   assume R[iir#g] == 0;
   assume 0 <= C[iir#g];
@@ -704,24 +758,6 @@ procedure iir#anon$5#exit#11()
   assume 0 <= C[iir#a];
   assume 0 <= R[iir#a];
   assume (171 * M[iir#g][-1]) == M[iir#f][0];
-  assume (forall i: int :: 
-    (0 <= i) && (i < (R[iir#b] + C[iir#b])) ==> (M[iir#b][i] == (85 * M[iir#a][i]))
-  );
-  assume (forall i: int :: 
-    (0 <= i) && (i < (R[iir#c] + C[iir#c])) ==> (M[iir#c][i] == (M[iir#b][i] + M[iir#f][i]))
-  );
-  assume (forall i: int :: 
-    (0 <= i) && (i < (R[iir#d] + C[iir#d])) ==> (M[iir#d][i] == AT#RShift(M[iir#c][i], 8))
-  );
-  assume (forall i: int :: 
-    (0 <= i) && (i < (R[iir#g] + C[iir#g])) ==> (M[iir#g][i] == AT#RShift(M[iir#c][i], 8))
-  );
-  assume (forall i: int :: 
-    (0 <= i) && (i < (R[iir#e] + C[iir#e])) ==> (M[iir#e][i] == (171 * M[iir#d][i]))
-  );
-  assume (forall i: int :: 
-    (1 <= i) && (i < (R[iir#f] + C[iir#f])) ==> (M[iir#f][i] == M[iir#e][i - 1])
-  );
   assume !(((((1 <= C[iir#e]) || (1 <= C[iir#a])) || (1 <= C[iir#d])) || (1 <= C[iir#c])) || ((1 <= C[iir#b]) && (1 <= C[iir#f])));
   assert {:msg "  23.3: The network might leave unread tokens on channel a"} C[iir#a] == 0;
   assert {:msg "  23.3: The network might leave unread tokens on channel b"} C[iir#b] == 0;
